@prefix : <http://purl.org/pan-science/ESRFET#> .
@prefix owl: <http://www.w3.org/2002/07/owl#> .
@prefix rdf: <http://www.w3.org/1999/02/22-rdf-syntax-ns#> .
@prefix xml: <http://www.w3.org/XML/1998/namespace> .
@prefix xsd: <http://www.w3.org/2001/XMLSchema#> .
@prefix rdfs: <http://www.w3.org/2000/01/rdf-schema#> .
@base <http://purl.org/pan-science/ESRFET#> .

<http://purl.org/pan-science/ESRFET> rdf:type owl:Ontology ;
                                      owl:imports <http://purl.org/pan-science/PaNET/PaNET.owl> ;
                                      <http://purl.org/dc/terms/abstract> "The ESRFET ontology describes beamline experimental techniques at ESRF to enhance the FAIRness of experimental metadata. It supports semantic interoperability and reasoning over relationships between techniques." ;
                                      <http://purl.org/dc/terms/created> "2025-07-07"^^xsd:date ;
                                      <http://purl.org/dc/terms/creator> <http://purl.org/pan-science/ESRFET#person/GKoumoutsos> ,
                                                                         <http://purl.org/pan-science/ESRFET#person/WDeNolf> ;
                                      <http://purl.org/dc/terms/license> <http://creativecommons.org/licenses/by/4.0/> ;
                                      <http://purl.org/dc/terms/modified> "2025-09-06"^^xsd:date ;
                                      <http://purl.org/dc/terms/title> "The ESRF Experimental Techniques Ontology"@en ;
                                      <http://purl.org/vocab/vann/preferredNamespacePrefix> "ESRFET"@en ;
                                      <http://purl.org/vocab/vann/preferredNamespaceUri> <http://purl.org/pan-science/ESRFET> ;
                                      rdfs:comment "The ESRF Ontologies project provides ontologies related to ESRF data acquisition."@en ;
                                      owl:versionInfo "v0.1.0" .

#################################################################
#    Annotation properties
#################################################################

###  http://purl.org/dc/terms/abstract
<http://purl.org/dc/terms/abstract> rdf:type owl:AnnotationProperty .


###  http://purl.org/dc/terms/created
<http://purl.org/dc/terms/created> rdf:type owl:AnnotationProperty .


###  http://purl.org/dc/terms/creator
<http://purl.org/dc/terms/creator> rdf:type owl:AnnotationProperty .


###  http://purl.org/dc/terms/license
<http://purl.org/dc/terms/license> rdf:type owl:AnnotationProperty .


###  http://purl.org/dc/terms/modified
<http://purl.org/dc/terms/modified> rdf:type owl:AnnotationProperty .


###  http://purl.org/dc/terms/title
<http://purl.org/dc/terms/title> rdf:type owl:AnnotationProperty .


###  http://purl.org/vocab/vann/preferredNamespacePrefix
<http://purl.org/vocab/vann/preferredNamespacePrefix> rdf:type owl:AnnotationProperty .


###  http://purl.org/vocab/vann/preferredNamespaceUri
<http://purl.org/vocab/vann/preferredNamespaceUri> rdf:type owl:AnnotationProperty .


###  http://www.w3.org/2004/02/skos/core#altLabel
<http://www.w3.org/2004/02/skos/core#altLabel> rdf:type owl:AnnotationProperty .


###  http://www.w3.org/2004/02/skos/core#prefLabel
<http://www.w3.org/2004/02/skos/core#prefLabel> rdf:type owl:AnnotationProperty .


###  http://xmlns.com/foaf/0.1/mbox
<http://xmlns.com/foaf/0.1/mbox> rdf:type owl:AnnotationProperty .


#################################################################
#    Datatypes
#################################################################

###  http://www.w3.org/2001/XMLSchema#date
xsd:date rdf:type rdfs:Datatype .


#################################################################
#    Object Properties
#################################################################

###  http://purl.org/pan-science/ESRFET#measures_as_a_function_of
:measures_as_a_function_of rdf:type owl:ObjectProperty ;
                           rdfs:domain :experimental_technique ;
                           rdfs:range :space_time ;
                           rdfs:comment """Example: XAS measures as function of incident X-ray photon energy
                X-ray absorption tomography measures as function of sample orientation
                Scanning Micro X-ray fluorescence measures as function of sample translation""" .


###  http://purl.org/pan-science/ESRFET#measures_interaction_result_property
:measures_interaction_result_property rdf:type owl:ObjectProperty ;
                                      rdfs:domain :experimental_technique ;
                                      rdfs:range :detected_cascade_of_events_property ;
                                      rdfs:comment "Example: XRF measures photon energy" .


###  http://purl.org/pan-science/ESRFET#measures_result_of_interaction
:measures_result_of_interaction rdf:type owl:ObjectProperty ;
                                rdfs:domain :experimental_technique ;
                                rdfs:range :cascade_of_events_being_detected ;
                                rdfs:comment "Example: XRF measures fluorscence" .


###  http://purl.org/pan-science/ESRFET#measures_transmission_with_detector_type
:measures_transmission_with_detector_type rdf:type owl:ObjectProperty ;
                                          rdfs:domain :transmission ;
                                          rdfs:range :detector_type .


###  http://purl.org/pan-science/ESRFET#measures_with_a_detector_type
:measures_with_a_detector_type rdf:type owl:ObjectProperty ;
                               rdfs:domain :experimental_technique ;
                               rdfs:range :detector_type .


###  http://purl.org/pan-science/ESRFET#requires_sample_input
:requires_sample_input rdf:type owl:ObjectProperty ;
                       rdfs:domain :experimental_technique ;
                       rdfs:range :sample_input ;
                       rdfs:comment "Example: Soft X-ray Absorption Spectroscopy uses soft X-ray as sample input" .


###  http://purl.org/pan-science/ESRFET#requires_sample_input_property
:requires_sample_input_property rdf:type owl:ObjectProperty ;
                                rdfs:domain :experimental_technique ;
                                rdfs:range :sample_input_property .


###  http://purl.org/pan-science/ESRFET#requires_sample_type
:requires_sample_type rdf:type owl:ObjectProperty ;
                      rdfs:domain :experimental_technique ;
                      rdfs:range :sample_type ;
                      rdfs:comment """Example: XRPD requires powder
                XRD does not require any sample type

                Another way of looking at it:
                diffraction (cascade of events being detected) requires 'any of' single crystal, powder, fiber
                X-ray powder diffraction (technique) requires 'exactly' powder""" .


#################################################################
#    Data properties
#################################################################

###  http://purl.org/pan-science/ESRFET#atomic_distance_resolution_unit
:atomic_distance_resolution_unit rdf:type owl:DatatypeProperty .


###  http://purl.org/pan-science/ESRFET#atomic_distance_unit
:atomic_distance_unit rdf:type owl:DatatypeProperty ;
                      rdfs:domain :diffraction_of_elastic_scattering ;
                      rdfs:range xsd:string .


###  http://purl.org/pan-science/ESRFET#energy_range_unit
:energy_range_unit rdf:type owl:DatatypeProperty ;
                   rdfs:range xsd:string ;
                   rdfs:label "has energy range unit" .


###  http://purl.org/pan-science/ESRFET#energy_range_value
:energy_range_value rdf:type owl:DatatypeProperty ;
                    rdfs:range xsd:float ;
                    rdfs:label "has energy range value" .


###  http://purl.org/pan-science/ESRFET#sample_spatial_resolution
:sample_spatial_resolution rdf:type owl:DatatypeProperty .


###  http://purl.org/pan-science/ESRFET#sample_spatial_resolution_unit
:sample_spatial_resolution_unit rdf:type owl:DatatypeProperty .


#################################################################
#    Classes
#################################################################

###  http://purl.org/pan-science/ESRFET#ARPES
:ARPES rdf:type owl:Class ;
       rdfs:subClassOf :experimental_technique ;
       rdfs:comment "Angle-Resolved Photoemission Spectroscopy (ARPES) measures the energy and momentum of electrons emitted from a sample when illuminated by photons, mapping the electronic band structure and Fermi surface of materials." ;
       rdfs:label "ARPES" ;
       <http://www.w3.org/2004/02/skos/core#prefLabel> "Angle-Resolved Photoemission Spectroscopy" .


###  http://purl.org/pan-science/ESRFET#BCDI
:BCDI rdf:type owl:Class ;
      rdfs:subClassOf :experimental_technique ;
      rdfs:comment "Bragg Coherent Diffraction Imaging (BCDI) measures the coherent diffraction around a Bragg peak from a crystalline sample to reconstruct the 3D shape and internal strain field of individual nanocrystals. The result is a high-resolution image of the crystalline structure and deformation." ;
      rdfs:label "BCDI" ;
      <http://www.w3.org/2004/02/skos/core#prefLabel> "Bragg Coherent Diffraction Imaging" .


###  http://purl.org/pan-science/ESRFET#BioSAXS
:BioSAXS rdf:type owl:Class ;
         owl:equivalentClass [ owl:intersectionOf ( :experimental_technique
                                                    [ rdf:type owl:Restriction ;
                                                      owl:onProperty :measures_interaction_result_property ;
                                                      owl:someValuesFrom :large_length_scales
                                                    ]
                                                    [ rdf:type owl:Restriction ;
                                                      owl:onProperty :measures_result_of_interaction ;
                                                      owl:someValuesFrom :diffraction_of_elastic_scattering
                                                    ]
                                                    [ rdf:type owl:Restriction ;
                                                      owl:onProperty :requires_sample_input ;
                                                      owl:someValuesFrom :x-ray
                                                    ]
                                                    [ rdf:type owl:Restriction ;
                                                      owl:onProperty :requires_sample_type ;
                                                      owl:someValuesFrom :biological_sample
                                                    ]
                                                  ) ;
                               rdf:type owl:Class
                             ] ;
         rdfs:comment "BioSAXS is SAXS applied to biological macromolecules in solution to determine their size, shape, flexibility, and aggregation state in near-native conditions." ;
         rdfs:label "BioSAXS" .


###  http://purl.org/pan-science/ESRFET#CDI
:CDI rdf:type owl:Class ;
     rdfs:subClassOf :experimental_technique ;
     rdfs:comment "Coherent Diffraction Imaging (CDI) measures the far-field diffraction pattern from a sample illuminated with a coherent X-ray beam. The image of the sample is reconstructed computationally from the diffraction data using phase retrieval algorithms, yielding high-resolution, lensless imaging of the electron density or scattering potential." ;
     rdfs:label "CDI" ;
     <http://www.w3.org/2004/02/skos/core#altLabel> "CXD" ,
                                                    "CXDI" ,
                                                    "Coherent X-ray Diffraction" ,
                                                    "Coherent X-ray Diffraction Imaging" ;
     <http://www.w3.org/2004/02/skos/core#prefLabel> "Coherent Diffraction Imaging" .


###  http://purl.org/pan-science/ESRFET#CMS
:CMS rdf:type owl:Class ;
     rdfs:subClassOf :experimental_technique ;
     rdfs:comment "Conventional Mössbauer Spectroscopy measures the resonant absorption of X-rays by Mössbauer-active nuclei (e.g. Fe-57) using a radioactive source scanned in velocity. It provides information on oxidation state, magnetic ordering, and local electronic and structural environment through hyperfine interactions." ;
     rdfs:label "CMS" ;
     <http://www.w3.org/2004/02/skos/core#prefLabel> "Conventional Mössbauer Spectroscopy" .


###  http://purl.org/pan-science/ESRFET#CRYO-EM
:CRYO-EM rdf:type owl:Class ;
         owl:equivalentClass [ owl:intersectionOf ( :experimental_technique
                                                    [ rdf:type owl:Restriction ;
                                                      owl:onProperty :measures_as_a_function_of ;
                                                      owl:someValuesFrom :detection_as_a_function_of_limited_number_of_sample_to_detector_distance
                                                    ]
                                                    [ rdf:type owl:Restriction ;
                                                      owl:onProperty :measures_as_a_function_of ;
                                                      owl:someValuesFrom :serial_screening
                                                    ]
                                                    [ rdf:type owl:Restriction ;
                                                      owl:onProperty :measures_as_a_function_of ;
                                                      owl:someValuesFrom :tomography
                                                    ]
                                                    [ rdf:type owl:Restriction ;
                                                      owl:onProperty :measures_result_of_interaction ;
                                                      owl:someValuesFrom :refraction
                                                    ]
                                                    [ rdf:type owl:Restriction ;
                                                      owl:onProperty :measures_result_of_interaction ;
                                                      owl:someValuesFrom :transmission
                                                    ]
                                                    [ rdf:type owl:Restriction ;
                                                      owl:onProperty :requires_sample_input ;
                                                      owl:someValuesFrom :electrons
                                                    ]
                                                    [ rdf:type owl:Restriction ;
                                                      owl:onProperty :requires_sample_input_property ;
                                                      owl:someValuesFrom :cryogenic_temperature
                                                    ]
                                                  ) ;
                               rdf:type owl:Class
                             ] ;
         rdfs:comment "Cryo-Electron Microscopy (Cryo-EM) measures phase shifts in electron waves transmitted through cryogenically preserved samples, producing high-contrast 2D images of biological macromolecules or soft materials at near-atomic resolution. Similar to serial crystallography, it reconstructs 3D structures from many randomly oriented single-particle images of identical molecules." ;
         rdfs:label "CRYO-EM" ;
         <http://www.w3.org/2004/02/skos/core#prefLabel> "Cryo-Electron Microscopy" .


###  http://purl.org/pan-science/ESRFET#CRYO-ET
:CRYO-ET rdf:type owl:Class ;
         owl:equivalentClass [ owl:intersectionOf ( :experimental_technique
                                                    [ rdf:type owl:Restriction ;
                                                      owl:onProperty :measures_as_a_function_of ;
                                                      owl:someValuesFrom :detection_as_a_function_of_limited_number_of_sample_to_detector_distance
                                                    ]
                                                    [ rdf:type owl:Restriction ;
                                                      owl:onProperty :measures_as_a_function_of ;
                                                      owl:someValuesFrom :individual_specimen
                                                    ]
                                                    [ rdf:type owl:Restriction ;
                                                      owl:onProperty :measures_as_a_function_of ;
                                                      owl:someValuesFrom :tomography
                                                    ]
                                                    [ rdf:type owl:Restriction ;
                                                      owl:onProperty :measures_result_of_interaction ;
                                                      owl:someValuesFrom :refraction
                                                    ]
                                                    [ rdf:type owl:Restriction ;
                                                      owl:onProperty :measures_result_of_interaction ;
                                                      owl:someValuesFrom :transmission
                                                    ]
                                                    [ rdf:type owl:Restriction ;
                                                      owl:onProperty :requires_sample_input ;
                                                      owl:someValuesFrom :electrons
                                                    ]
                                                    [ rdf:type owl:Restriction ;
                                                      owl:onProperty :requires_sample_input_property ;
                                                      owl:someValuesFrom :cryogenic_temperature
                                                    ]
                                                  ) ;
                               rdf:type owl:Class
                             ] ;
         rdfs:comment "Cryo-Electron Tomography (Cryo-ET) measures phase shifts in transmitted electrons from multiple tilt angles of a cryogenically preserved sample to reconstruct 3D structures of cells or macromolecular assemblies with enhanced contrast and nanometer resolution." ;
         rdfs:label "CRYO-ET" ;
         <http://www.w3.org/2004/02/skos/core#prefLabel> "Cryo-Electron Tomography" .


###  http://purl.org/pan-science/ESRFET#CT
:CT rdf:type owl:Class ;
    owl:equivalentClass [ owl:intersectionOf ( :experimental_technique
                                               [ rdf:type owl:Restriction ;
                                                 owl:onProperty :measures_as_a_function_of ;
                                                 owl:someValuesFrom :tomography
                                               ]
                                             ) ;
                          rdf:type owl:Class
                        ] ;
    rdfs:comment "Computed Tomography (CT) measures projections of radiation (such as X-rays, electrons, or neutrons) through a sample from multiple angles and reconstructs 3D internal maps of material properties, providing structural information whose contrast depends on the measured interaction (e.g., absorption, phase, fluorescence, or diffraction)." ;
    rdfs:label "CT" ;
    <http://www.w3.org/2004/02/skos/core#prefLabel> "Computed Tomography" .


###  http://purl.org/pan-science/ESRFET#CXDI
:CXDI rdf:type owl:Class ;
      rdfs:subClassOf :experimental_technique ;
      rdfs:comment "Coherent X-ray Diffraction Imaging (CXDI) measures the coherent X-ray diffraction pattern from an isolated object or nanostructure. The 3D electron density is reconstructed computationally using phase retrieval, providing high-resolution, lensless imaging of the sample's internal structure." ;
      rdfs:label "CXDI" ;
      <http://www.w3.org/2004/02/skos/core#prefLabel> "Coherent X-ray Diffraction Imaging" .


###  http://purl.org/pan-science/ESRFET#DAC
:DAC rdf:type owl:Class ;
     rdfs:subClassOf :sample_input ;
     rdfs:comment "Diamond Anvil Cell to apply pressure on the sample" .


###  http://purl.org/pan-science/ESRFET#DAFS
:DAFS rdf:type owl:Class ;
      rdfs:subClassOf :experimental_technique ;
      rdfs:comment "Diffraction Anomalous Fine Structure (DAFS) measures the intensity of Bragg diffraction as a function of X-ray photon energy near an absorption edge. It combines diffraction and XAS to provide element-specific structural information, such as site occupancy, bonding environment, and local distortions in crystals." ;
      rdfs:label "DAFS" ;
      <http://www.w3.org/2004/02/skos/core#prefLabel> "Diffraction Anomalous Fine Structure" .


###  http://purl.org/pan-science/ESRFET#DCT
:DCT rdf:type owl:Class ;
     owl:equivalentClass [ owl:intersectionOf ( :experimental_technique
                                                [ rdf:type owl:Restriction ;
                                                  owl:onProperty :measures_as_a_function_of ;
                                                  owl:someValuesFrom :tomography
                                                ]
                                                [ rdf:type owl:Restriction ;
                                                  owl:onProperty :measures_result_of_interaction ;
                                                  owl:someValuesFrom :diffraction_of_elastic_scattering
                                                ]
                                                [ rdf:type owl:Restriction ;
                                                  owl:onProperty :measures_result_of_interaction ;
                                                  owl:someValuesFrom [ rdf:type owl:Restriction ;
                                                                       owl:onProperty :measures_transmission_with_detector_type ;
                                                                       owl:someValuesFrom :area_detector
                                                                     ]
                                                ]
                                                [ rdf:type owl:Restriction ;
                                                  owl:onProperty :requires_sample_input ;
                                                  owl:someValuesFrom :x-ray
                                                ]
                                                [ rdf:type owl:Restriction ;
                                                  owl:onProperty :requires_sample_type ;
                                                  owl:someValuesFrom :polycrystalline_sample
                                                ]
                                              ) ;
                           rdf:type owl:Class
                         ] ;
     rdfs:comment "DCT is a near-field diffraction-based imaging technique that provides high-resolution grain maps of polycrystalline materials (Ludwig et al. 2008). For each individual grain, the technique can provide orientation and average elastic strain tensor components with an accuracy of a few times 1e-4 (Reischig et al. 2013). The technique combines the concepts of image reconstruction from projections (tomography) and X-ray diffraction imaging (topography)." ;
     rdfs:label "DCT" ;
     <http://www.w3.org/2004/02/skos/core#prefLabel> "Diffraction Contrast Tomography" .


###  http://purl.org/pan-science/ESRFET#DFXM
:DFXM rdf:type owl:Class ;
      rdfs:subClassOf :experimental_technique ;
      rdfs:comment "Dark-Field X-ray Microscopy (DFXM) measures X-ray diffraction in a dark-field imaging geometry to map crystalline structure, orientation, strain, and defects in 3D within bulk materials. It provides spatially resolved imaging of internal microstructures at micrometer to sub-micrometer resolution." ;
      rdfs:label "DFXM" ;
      <http://www.w3.org/2004/02/skos/core#prefLabel> "Dark-Field X-ray Microscopy" .


###  http://purl.org/pan-science/ESRFET#ED-EXAFS
:ED-EXAFS rdf:type owl:Class ;
          owl:equivalentClass [ owl:intersectionOf ( :experimental_technique
                                                     [ rdf:type owl:Restriction ;
                                                       owl:onProperty :measures_as_a_function_of ;
                                                       owl:someValuesFrom :extended
                                                     ]
                                                     [ rdf:type owl:Restriction ;
                                                       owl:onProperty :measures_interaction_result_property ;
                                                       owl:someValuesFrom :photon_count
                                                     ]
                                                     [ rdf:type owl:Restriction ;
                                                       owl:onProperty :measures_result_of_interaction ;
                                                       owl:someValuesFrom :atomic_core_excitation
                                                     ]
                                                     [ rdf:type owl:Restriction ;
                                                       owl:onProperty :requires_sample_input ;
                                                       owl:someValuesFrom :x-ray
                                                     ]
                                                     [ rdf:type owl:Restriction ;
                                                       owl:onProperty :requires_sample_input_property ;
                                                       owl:someValuesFrom :disperse_incident_energy_in_space
                                                     ]
                                                   ) ;
                                rdf:type owl:Class
                              ] ;
          rdfs:comment "Energy Dispersive Extended X-ray Absorption Fine Structure (ED-EXAFS) measures oscillations in X-ray absorption probability beyond the edge with energy-dispersive detection, providing local atomic structural information such as bond distances and coordination numbers, acquired quickly without angular scanning." ;
          rdfs:label "ED-EXAFS" ;
          <http://www.w3.org/2004/02/skos/core#prefLabel> "Energy Dispersive Extended X-ray Absorption Fine Structure" .


###  http://purl.org/pan-science/ESRFET#ED-XANES
:ED-XANES rdf:type owl:Class ;
          owl:equivalentClass [ owl:intersectionOf ( :experimental_technique
                                                     [ rdf:type owl:Restriction ;
                                                       owl:onProperty :measures_as_a_function_of ;
                                                       owl:someValuesFrom :near_edge
                                                     ]
                                                     [ rdf:type owl:Restriction ;
                                                       owl:onProperty :measures_interaction_result_property ;
                                                       owl:someValuesFrom :photon_count
                                                     ]
                                                     [ rdf:type owl:Restriction ;
                                                       owl:onProperty :measures_result_of_interaction ;
                                                       owl:someValuesFrom :atomic_core_excitation
                                                     ]
                                                     [ rdf:type owl:Restriction ;
                                                       owl:onProperty :requires_sample_input ;
                                                       owl:someValuesFrom :x-ray
                                                     ]
                                                     [ rdf:type owl:Restriction ;
                                                       owl:onProperty :requires_sample_input_property ;
                                                       owl:someValuesFrom :disperse_incident_energy_in_space
                                                     ]
                                                   ) ;
                                rdf:type owl:Class
                              ] ;
          rdfs:comment "Energy Dispersive X-ray Absorption Near Edge Structure (ED-XANES) measures the X-ray absorption probability near the absorption edge using energy-dispersive detection, providing rapid information about the oxidation state and electronic structure without scanning incident energy." ;
          rdfs:label "ED-XANES" ;
          <http://www.w3.org/2004/02/skos/core#prefLabel> "Energy Dispersive X-ray Absorption Near Edge Structure" .


###  http://purl.org/pan-science/ESRFET#ED-XAS
:ED-XAS rdf:type owl:Class ;
        owl:equivalentClass [ owl:intersectionOf ( :experimental_technique
                                                   [ rdf:type owl:Restriction ;
                                                     owl:onProperty :measures_as_a_function_of ;
                                                     owl:someValuesFrom :detection_as_a_function_of_incident_energy
                                                   ]
                                                   [ rdf:type owl:Restriction ;
                                                     owl:onProperty :measures_interaction_result_property ;
                                                     owl:someValuesFrom :photon_count
                                                   ]
                                                   [ rdf:type owl:Restriction ;
                                                     owl:onProperty :measures_result_of_interaction ;
                                                     owl:someValuesFrom :atomic_core_excitation
                                                   ]
                                                   [ rdf:type owl:Restriction ;
                                                     owl:onProperty :requires_sample_input ;
                                                     owl:someValuesFrom :x-ray
                                                   ]
                                                   [ rdf:type owl:Restriction ;
                                                     owl:onProperty :requires_sample_input_property ;
                                                     owl:someValuesFrom :disperse_incident_energy_in_space
                                                   ]
                                                 ) ;
                              rdf:type owl:Class
                            ] ;
        rdfs:comment "Energy Dispersive X-ray Absorption Spectroscopy (ED-XAS) measures X-ray absorption as a function of energy simultaneously by dispersing the X-ray beam in space with a polychromatic source and position-sensitive detector, enabling rapid acquisition of absorption spectra without scanning the incident energy." ;
        rdfs:label "ED-XAS" ;
        <http://www.w3.org/2004/02/skos/core#prefLabel> "Energy Dispersive X-ray Absorption Spectroscopy" .


###  http://purl.org/pan-science/ESRFET#ED-XRD
:ED-XRD rdf:type owl:Class ;
        owl:equivalentClass [ owl:intersectionOf ( :experimental_technique
                                                   [ rdf:type owl:Restriction ;
                                                     owl:onProperty :measures_interaction_result_property ;
                                                     owl:someValuesFrom :photon_energy
                                                   ]
                                                   [ rdf:type owl:Restriction ;
                                                     owl:onProperty :measures_result_of_interaction ;
                                                     owl:someValuesFrom :diffraction_of_elastic_scattering
                                                   ]
                                                   [ rdf:type owl:Restriction ;
                                                     owl:onProperty :measures_with_a_detector_type ;
                                                     owl:someValuesFrom :energy_dispersive_detector
                                                   ]
                                                   [ rdf:type owl:Restriction ;
                                                     owl:onProperty :requires_sample_input ;
                                                     owl:someValuesFrom :x-ray
                                                   ]
                                                 ) ;
                              rdf:type owl:Class
                            ] ;
        rdfs:comment "Energy Dispersive X-ray Diffraction (ED-XRD) measures diffraction patterns of a sample by detecting diffracted X-rays at a fixed angle while dispersing their energies, enabling fast phase identification and structural analysis without angular scanning." ;
        rdfs:label "ED-XRD" ;
        <http://www.w3.org/2004/02/skos/core#prefLabel> "Energy Dispersive X-ray Diffraction" .


###  http://purl.org/pan-science/ESRFET#ED-XRF
:ED-XRF rdf:type owl:Class ;
        owl:equivalentClass [ owl:intersectionOf ( :experimental_technique
                                                   [ rdf:type owl:Restriction ;
                                                     owl:onProperty :measures_interaction_result_property ;
                                                     owl:someValuesFrom :photon_count
                                                   ]
                                                   [ rdf:type owl:Restriction ;
                                                     owl:onProperty :measures_interaction_result_property ;
                                                     owl:someValuesFrom :photon_energy
                                                   ]
                                                   [ rdf:type owl:Restriction ;
                                                     owl:onProperty :measures_result_of_interaction ;
                                                     owl:someValuesFrom :fluorescence
                                                   ]
                                                   [ rdf:type owl:Restriction ;
                                                     owl:onProperty :measures_with_a_detector_type ;
                                                     owl:someValuesFrom :energy_dispersive_detector
                                                   ]
                                                   [ rdf:type owl:Restriction ;
                                                     owl:onProperty :requires_sample_input ;
                                                     owl:someValuesFrom :x-ray
                                                   ]
                                                 ) ;
                              rdf:type owl:Class
                            ] ;
        rdfs:comment "Energy Dispersive X-ray Fluorescence Spectroscopy (ED-XRF) measures the energies of fluorescent X-rays emitted by a sample excited by a broad-spectrum X-ray source, providing elemental composition analysis without scanning the incident energy." ;
        rdfs:label "ED-XRF" ;
        <http://www.w3.org/2004/02/skos/core#prefLabel> "Energy Dispersive X-ray Fluorescence Spectroscopy" .


###  http://purl.org/pan-science/ESRFET#ED-XRPD
:ED-XRPD rdf:type owl:Class ;
         owl:equivalentClass [ owl:intersectionOf ( :experimental_technique
                                                    [ rdf:type owl:Restriction ;
                                                      owl:onProperty :measures_interaction_result_property ;
                                                      owl:someValuesFrom :photon_energy
                                                    ]
                                                    [ rdf:type owl:Restriction ;
                                                      owl:onProperty :measures_result_of_interaction ;
                                                      owl:someValuesFrom :diffraction_of_elastic_scattering
                                                    ]
                                                    [ rdf:type owl:Restriction ;
                                                      owl:onProperty :measures_with_a_detector_type ;
                                                      owl:someValuesFrom :energy_dispersive_detector
                                                    ]
                                                    [ rdf:type owl:Restriction ;
                                                      owl:onProperty :requires_sample_input ;
                                                      owl:someValuesFrom :x-ray
                                                    ]
                                                    [ rdf:type owl:Restriction ;
                                                      owl:onProperty :requires_sample_type ;
                                                      owl:someValuesFrom :powder_sample
                                                    ]
                                                  ) ;
                               rdf:type owl:Class
                             ] ;
         rdfs:comment "Energy Dispersive X-ray Powder Diffraction (ED-XRPD) measures diffraction patterns of powdered samples by detecting diffracted X-rays at a fixed angle while varying their energy, enabling rapid phase identification and structural analysis without scanning angles." ;
         rdfs:label "ED-XRPD" ;
         <http://www.w3.org/2004/02/skos/core#prefLabel> "Energy Dispersive X-ray Powder Diffraction" .


###  http://purl.org/pan-science/ESRFET#EDS
:EDS rdf:type owl:Class ;
     owl:equivalentClass [ owl:intersectionOf ( :experimental_technique
                                                [ rdf:type owl:Restriction ;
                                                  owl:onProperty :measures_interaction_result_property ;
                                                  owl:someValuesFrom :photon_count
                                                ]
                                                [ rdf:type owl:Restriction ;
                                                  owl:onProperty :measures_interaction_result_property ;
                                                  owl:someValuesFrom :photon_energy
                                                ]
                                                [ rdf:type owl:Restriction ;
                                                  owl:onProperty :measures_result_of_interaction ;
                                                  owl:someValuesFrom :fluorescence
                                                ]
                                                [ rdf:type owl:Restriction ;
                                                  owl:onProperty :measures_with_a_detector_type ;
                                                  owl:someValuesFrom :energy_dispersive_detector
                                                ]
                                                [ rdf:type owl:Restriction ;
                                                  owl:onProperty :requires_sample_input ;
                                                  owl:someValuesFrom :electrons
                                                ]
                                              ) ;
                           rdf:type owl:Class
                         ] ;
     rdfs:comment "EDS measures X-ray photons coming from a sample during electron irradition  with an energy dispersive detector and derives elemental composition from the energy of the fluorescence photons" ;
     rdfs:label "EDS" ;
     <http://www.w3.org/2004/02/skos/core#prefLabel> "Energy Dispersive X-ray Spectroscopy" .


###  http://purl.org/pan-science/ESRFET#EM
:EM rdf:type owl:Class ;
    owl:equivalentClass [ owl:intersectionOf ( :experimental_technique
                                               [ rdf:type owl:Restriction ;
                                                 owl:onProperty :requires_sample_input ;
                                                 owl:someValuesFrom :electrons
                                               ]
                                             ) ;
                          rdf:type owl:Class
                        ] ;
    rdfs:comment "Electron Microscopy (EM) uses a beam of electrons as illumination, controlled by electron optics analogous to glass lenses in light microscopes, to measure electron scattering or transmission through a sample. This technique provides high-resolution images and electron diffraction patterns, revealing structural, morphological, and compositional information at nanometer to atomic scales." ;
    rdfs:label "EM" ;
    <http://www.w3.org/2004/02/skos/core#prefLabel> "Electron Microscopy" .


###  http://purl.org/pan-science/ESRFET#EXAFS
:EXAFS rdf:type owl:Class ;
       owl:equivalentClass [ owl:intersectionOf ( :experimental_technique
                                                  [ rdf:type owl:Restriction ;
                                                    owl:onProperty :measures_as_a_function_of ;
                                                    owl:someValuesFrom :extended
                                                  ]
                                                  [ rdf:type owl:Restriction ;
                                                    owl:onProperty :measures_interaction_result_property ;
                                                    owl:someValuesFrom :photon_count
                                                  ]
                                                  [ rdf:type owl:Restriction ;
                                                    owl:onProperty :measures_result_of_interaction ;
                                                    owl:someValuesFrom :atomic_core_excitation
                                                  ]
                                                  [ rdf:type owl:Restriction ;
                                                    owl:onProperty :requires_sample_input ;
                                                    owl:someValuesFrom :x-ray
                                                  ]
                                                ) ;
                             rdf:type owl:Class
                           ] ;
       rdfs:comment "Extended X-ray Absorption Fine Structure (EXAFS) measures oscillations in X-ray absorption above an element’s absorption edge, providing information on the local atomic environment, including distances, coordination numbers, and disorder around the absorbing atoms." ;
       rdfs:label "EXAFS" ;
       <http://www.w3.org/2004/02/skos/core#prefLabel> "Extended X-ray Absorption Fine Structure" .


###  http://purl.org/pan-science/ESRFET#FF-EXAFS
:FF-EXAFS rdf:type owl:Class ;
          owl:equivalentClass [ owl:intersectionOf ( :experimental_technique
                                                     [ rdf:type owl:Restriction ;
                                                       owl:onProperty :measures_as_a_function_of ;
                                                       owl:someValuesFrom :extended
                                                     ]
                                                     [ rdf:type owl:Restriction ;
                                                       owl:onProperty :measures_as_a_function_of ;
                                                       owl:someValuesFrom :full-field_imaging
                                                     ]
                                                     [ rdf:type owl:Restriction ;
                                                       owl:onProperty :measures_interaction_result_property ;
                                                       owl:someValuesFrom :photon_count
                                                     ]
                                                     [ rdf:type owl:Restriction ;
                                                       owl:onProperty :measures_result_of_interaction ;
                                                       owl:someValuesFrom :atomic_core_excitation
                                                     ]
                                                     [ rdf:type owl:Restriction ;
                                                       owl:onProperty :requires_sample_input ;
                                                       owl:someValuesFrom :x-ray
                                                     ]
                                                   ) ;
                                rdf:type owl:Class
                              ] ;
          rdfs:comment "FF-EXAFS measures the extended region of the absorption spectrum across a 2D sample area using broad X-ray beam and an area detector, providing spatially resolved information on local atomic structure, such as bond lengths and coordination." ;
          rdfs:label "FF-EXAFS" ;
          <http://www.w3.org/2004/02/skos/core#prefLabel> "Full-Field Extended X-ray Absorption Fine Structure Imaging" .


###  http://purl.org/pan-science/ESRFET#FF-XANES
:FF-XANES rdf:type owl:Class ;
          owl:equivalentClass [ owl:intersectionOf ( :experimental_technique
                                                     [ rdf:type owl:Restriction ;
                                                       owl:onProperty :measures_as_a_function_of ;
                                                       owl:someValuesFrom :full-field_imaging
                                                     ]
                                                     [ rdf:type owl:Restriction ;
                                                       owl:onProperty :measures_as_a_function_of ;
                                                       owl:someValuesFrom :near_edge
                                                     ]
                                                     [ rdf:type owl:Restriction ;
                                                       owl:onProperty :measures_interaction_result_property ;
                                                       owl:someValuesFrom :photon_count
                                                     ]
                                                     [ rdf:type owl:Restriction ;
                                                       owl:onProperty :measures_result_of_interaction ;
                                                       owl:someValuesFrom :atomic_core_excitation
                                                     ]
                                                     [ rdf:type owl:Restriction ;
                                                       owl:onProperty :requires_sample_input ;
                                                       owl:someValuesFrom :x-ray
                                                     ]
                                                   ) ;
                                rdf:type owl:Class
                              ] ;
          rdfs:comment "FF-XANES measures the near-edge region of the absorption spectrum across a 2D sample area using broad X-ray beam and an area detector, providing spatially resolved information on chemical state and electronic structure." ;
          rdfs:label "FF-XANES" ;
          <http://www.w3.org/2004/02/skos/core#prefLabel> "Full‑Field X-ray Absorption Near Edge Structure Imaging" .


###  http://purl.org/pan-science/ESRFET#FF-XAS
:FF-XAS rdf:type owl:Class ;
        owl:equivalentClass [ owl:intersectionOf ( :experimental_technique
                                                   [ rdf:type owl:Restriction ;
                                                     owl:onProperty :measures_as_a_function_of ;
                                                     owl:someValuesFrom :detection_as_a_function_of_incident_energy
                                                   ]
                                                   [ rdf:type owl:Restriction ;
                                                     owl:onProperty :measures_as_a_function_of ;
                                                     owl:someValuesFrom :full-field_imaging
                                                   ]
                                                   [ rdf:type owl:Restriction ;
                                                     owl:onProperty :measures_interaction_result_property ;
                                                     owl:someValuesFrom :photon_count
                                                   ]
                                                   [ rdf:type owl:Restriction ;
                                                     owl:onProperty :measures_result_of_interaction ;
                                                     owl:someValuesFrom :atomic_core_excitation
                                                   ]
                                                   [ rdf:type owl:Restriction ;
                                                     owl:onProperty :requires_sample_input ;
                                                     owl:someValuesFrom :x-ray
                                                   ]
                                                 ) ;
                              rdf:type owl:Class
                            ] ;
        rdfs:comment "FF-XAS measures X-ray absorption spectra across a 2D sample area using broad X-ray beam and an area detector, providing spatially resolved insight into electronic and atomic structure." ;
        rdfs:label "FF-XAS" ;
        <http://www.w3.org/2004/02/skos/core#prefLabel> "Full-Field X-ray Absorption Spectroscopy Imaging" .


###  http://purl.org/pan-science/ESRFET#FF-XRF
:FF-XRF rdf:type owl:Class ;
        owl:equivalentClass [ owl:intersectionOf ( :experimental_technique
                                                   [ rdf:type owl:Restriction ;
                                                     owl:onProperty :measures_as_a_function_of ;
                                                     owl:someValuesFrom :full-field_imaging
                                                   ]
                                                   [ rdf:type owl:Restriction ;
                                                     owl:onProperty :measures_interaction_result_property ;
                                                     owl:someValuesFrom :photon_count
                                                   ]
                                                   [ rdf:type owl:Restriction ;
                                                     owl:onProperty :measures_interaction_result_property ;
                                                     owl:someValuesFrom :photon_energy
                                                   ]
                                                   [ rdf:type owl:Restriction ;
                                                     owl:onProperty :measures_result_of_interaction ;
                                                     owl:someValuesFrom :fluorescence
                                                   ]
                                                   [ rdf:type owl:Restriction ;
                                                     owl:onProperty :measures_with_a_detector_type ;
                                                     owl:someValuesFrom :area_detector
                                                   ]
                                                   [ rdf:type owl:Restriction ;
                                                     owl:onProperty :requires_sample_input ;
                                                     owl:someValuesFrom :x-ray
                                                   ]
                                                 ) ;
                              rdf:type owl:Class
                            ] ;
        rdfs:comment "FF-XRF measures X-ray fluorescence spectra across a 2D sample area using broad X-ray beam and an area detector, providing 2D elemental distribution maps in projection." ;
        rdfs:label "FF-XRF" ;
        <http://www.w3.org/2004/02/skos/core#prefLabel> "Full-Field X-ray Fluorescence Imaging" .


###  http://purl.org/pan-science/ESRFET#FS-EXAFS
:FS-EXAFS rdf:type owl:Class ;
          owl:equivalentClass [ owl:intersectionOf ( :experimental_technique
                                                     [ rdf:type owl:Restriction ;
                                                       owl:onProperty :measures_as_a_function_of ;
                                                       owl:someValuesFrom :extended
                                                     ]
                                                     [ rdf:type owl:Restriction ;
                                                       owl:onProperty :measures_as_a_function_of ;
                                                       owl:someValuesFrom :scanning_imaging
                                                     ]
                                                     [ rdf:type owl:Restriction ;
                                                       owl:onProperty :measures_interaction_result_property ;
                                                       owl:someValuesFrom :photon_count
                                                     ]
                                                     [ rdf:type owl:Restriction ;
                                                       owl:onProperty :measures_result_of_interaction ;
                                                       owl:someValuesFrom :atomic_core_excitation
                                                     ]
                                                     [ rdf:type owl:Restriction ;
                                                       owl:onProperty :requires_sample_input ;
                                                       owl:someValuesFrom :x-ray
                                                     ]
                                                   ) ;
                                rdf:type owl:Class
                              ] ;
          rdfs:comment "FS-EXAFS measures the extended region of the absorption spectrum across a 2D sample area using a focused X-ray beam, providing spatially resolved information on local atomic structure, such as bond lengths and coordination." ;
          rdfs:label "FS-EXAFS" ;
          <http://www.w3.org/2004/02/skos/core#prefLabel> "Full-Spectral Extended X-ray Absorption Fine Structure Imaging" .


###  http://purl.org/pan-science/ESRFET#FS-XAS
:FS-XAS rdf:type owl:Class ;
        owl:equivalentClass [ owl:intersectionOf ( :experimental_technique
                                                   [ rdf:type owl:Restriction ;
                                                     owl:onProperty :measures_as_a_function_of ;
                                                     owl:someValuesFrom :detection_as_a_function_of_incident_energy
                                                   ]
                                                   [ rdf:type owl:Restriction ;
                                                     owl:onProperty :measures_as_a_function_of ;
                                                     owl:someValuesFrom :scanning_imaging
                                                   ]
                                                   [ rdf:type owl:Restriction ;
                                                     owl:onProperty :measures_interaction_result_property ;
                                                     owl:someValuesFrom :photon_count
                                                   ]
                                                   [ rdf:type owl:Restriction ;
                                                     owl:onProperty :measures_result_of_interaction ;
                                                     owl:someValuesFrom :atomic_core_excitation
                                                   ]
                                                   [ rdf:type owl:Restriction ;
                                                     owl:onProperty :requires_sample_input ;
                                                     owl:someValuesFrom :x-ray
                                                   ]
                                                 ) ;
                              rdf:type owl:Class
                            ] ;
        rdfs:comment "FS-XAS measures X-ray absorption spectra across a 2D sample area using a focused X-ray beam, providing spatially resolved insight into electronic and atomic structure." ;
        rdfs:label "FS-XAS" ;
        <http://www.w3.org/2004/02/skos/core#prefLabel> "Full-Spectral X-ray Absorption Spectroscopy Imaging" .


###  http://purl.org/pan-science/ESRFET#FTIR
:FTIR rdf:type owl:Class ;
      owl:equivalentClass [ owl:intersectionOf ( :experimental_technique
                                                 [ rdf:type owl:Restriction ;
                                                   owl:onProperty :measures_result_of_interaction ;
                                                   owl:someValuesFrom :transmission
                                                 ]
                                                 [ rdf:type owl:Restriction ;
                                                   owl:onProperty :requires_sample_input ;
                                                   owl:someValuesFrom :infrared
                                                 ]
                                               ) ;
                            rdf:type owl:Class
                          ] ;
      rdfs:comment "Fourier Transform Infrared Spectroscopy (FTIR) measures the absorption of infrared light by a sample as a function of wavelength, providing information on molecular vibrations and chemical bonds to identify and characterize materials." ;
      rdfs:label "FTIR" ;
      <http://www.w3.org/2004/02/skos/core#prefLabel> "Fourier Transform Infrared Spectroscopy" .


###  http://purl.org/pan-science/ESRFET#GISAXS
:GISAXS rdf:type owl:Class ;
        owl:equivalentClass [ owl:intersectionOf ( :experimental_technique
                                                   [ rdf:type owl:Restriction ;
                                                     owl:onProperty :measures_interaction_result_property ;
                                                     owl:someValuesFrom :large_length_scales
                                                   ]
                                                   [ rdf:type owl:Restriction ;
                                                     owl:onProperty :measures_result_of_interaction ;
                                                     owl:someValuesFrom :diffraction_of_elastic_scattering
                                                   ]
                                                   [ rdf:type owl:Restriction ;
                                                     owl:onProperty :requires_sample_input ;
                                                     owl:someValuesFrom :x-ray
                                                   ]
                                                   [ rdf:type owl:Restriction ;
                                                     owl:onProperty :requires_sample_input_property ;
                                                     owl:someValuesFrom :sample_incident_angle_smaller_than_critical_angle
                                                   ]
                                                 ) ;
                              rdf:type owl:Class
                            ] ;
        rdfs:comment "Grazing-Incidence Small-Angle X-ray Scattering (GISAXS) measures scattered X-rays at small angles from a sample surface under shallow incidence, providing nanoscale information about thin film and surface morphology, including size, shape, and arrangement of nanostructures." ;
        rdfs:label "GISAXS" ;
        <http://www.w3.org/2004/02/skos/core#prefLabel> "Grazing Incidence Small Angle X-ray Scattering" .


###  http://purl.org/pan-science/ESRFET#GIWAXS
:GIWAXS rdf:type owl:Class ;
        owl:equivalentClass [ owl:intersectionOf ( :experimental_technique
                                                   [ rdf:type owl:Restriction ;
                                                     owl:onProperty :measures_interaction_result_property ;
                                                     owl:someValuesFrom :small_length_scales
                                                   ]
                                                   [ rdf:type owl:Restriction ;
                                                     owl:onProperty :measures_result_of_interaction ;
                                                     owl:someValuesFrom :diffraction_of_elastic_scattering
                                                   ]
                                                   [ rdf:type owl:Restriction ;
                                                     owl:onProperty :requires_sample_input ;
                                                     owl:someValuesFrom :x-ray
                                                   ]
                                                   [ rdf:type owl:Restriction ;
                                                     owl:onProperty :requires_sample_input_property ;
                                                     owl:someValuesFrom :sample_incident_angle_smaller_than_critical_angle
                                                   ]
                                                 ) ;
                              rdf:type owl:Class
                            ] ;
        rdfs:comment "Grazing-Incidence Wide-Angle X-ray Scattering (GIWAXS) measures scattered X-rays at wide angles under shallow incidence, providing information on molecular packing, crystalline order, and orientation in thin films and surfaces." ;
        rdfs:label "GIWAXS" ;
        <http://www.w3.org/2004/02/skos/core#prefLabel> "Grazing Incidence Wide Angle X-ray Scattering" .


###  http://purl.org/pan-science/ESRFET#GIXRD
:GIXRD rdf:type owl:Class ;
       owl:equivalentClass [ owl:intersectionOf ( :experimental_technique
                                                  [ rdf:type owl:Restriction ;
                                                    owl:onProperty :measures_result_of_interaction ;
                                                    owl:someValuesFrom :diffraction_of_elastic_scattering
                                                  ]
                                                  [ rdf:type owl:Restriction ;
                                                    owl:onProperty :requires_sample_input ;
                                                    owl:someValuesFrom :x-ray
                                                  ]
                                                  [ rdf:type owl:Restriction ;
                                                    owl:onProperty :requires_sample_input_property ;
                                                    owl:someValuesFrom :sample_incident_angle_smaller_than_critical_angle
                                                  ]
                                                ) ;
                             rdf:type owl:Class
                           ] ;
       rdfs:comment "Grazing-Incidence X-ray Diffraction (GIXRD) measures diffraction patterns from a sample surface using X-rays at shallow incident angles, providing structural information on thin films, surfaces, and near-surface regions, including phase composition and strain." ;
       rdfs:label "GIXRD" ;
       <http://www.w3.org/2004/02/skos/core#prefLabel> "Grazing Incidence X-ray Diffraction" .


###  http://purl.org/pan-science/ESRFET#HAXPES
:HAXPES rdf:type owl:Class ;
        rdfs:subClassOf :experimental_technique ;
        rdfs:comment "Hard X-ray Photoelectron Spectroscopy (HAXPES) uses high-energy X-rays to probe deeper into materials than conventional XPS, giving bulk-sensitive chemical and electronic information." ;
        rdfs:label "HAXPES" ;
        <http://www.w3.org/2004/02/skos/core#prefLabel> "Hard X-ray Photoelectron Spectroscopy" .


###  http://purl.org/pan-science/ESRFET#HERFD-XAS
:HERFD-XAS rdf:type owl:Class ;
           owl:equivalentClass [ owl:intersectionOf ( :experimental_technique
                                                      [ rdf:type owl:Restriction ;
                                                        owl:onProperty :measures_as_a_function_of ;
                                                        owl:someValuesFrom :detection_as_a_function_of_incident_energy
                                                      ]
                                                      [ rdf:type owl:Restriction ;
                                                        owl:onProperty :measures_interaction_result_property ;
                                                        owl:someValuesFrom :photon_count
                                                      ]
                                                      [ rdf:type owl:Restriction ;
                                                        owl:onProperty :measures_result_of_interaction ;
                                                        owl:someValuesFrom :atomic_core_excitation
                                                      ]
                                                      [ rdf:type owl:Restriction ;
                                                        owl:onProperty :measures_result_of_interaction ;
                                                        owl:someValuesFrom :fluorescence
                                                      ]
                                                      [ rdf:type owl:Restriction ;
                                                        owl:onProperty :requires_sample_input ;
                                                        owl:someValuesFrom :x-ray
                                                      ]
                                                    ) ;
                                 rdf:type owl:Class
                               ] ;
           rdfs:comment "High-Energy Resolution Fluorescence Detected X-ray Absorption Spectroscopy (HERFD-XAS) measures X-ray absorption using fluorescence detected with high energy resolution, enhancing spectral detail by reducing core-hole lifetime broadening to reveal subtle electronic and chemical state information." ;
           rdfs:label "HERFD-XAS" ;
           <http://www.w3.org/2004/02/skos/core#altLabel> "HERFD" ;
           <http://www.w3.org/2004/02/skos/core#prefLabel> "High-Energy Resolution Fluorescence Detected X-ray Absorption Spectroscopy" .


###  http://purl.org/pan-science/ESRFET#HP-XRD
:HP-XRD rdf:type owl:Class ;
        owl:equivalentClass [ owl:intersectionOf ( :experimental_technique
                                                   [ rdf:type owl:Restriction ;
                                                     owl:onProperty :measures_result_of_interaction ;
                                                     owl:someValuesFrom :diffraction_of_elastic_scattering
                                                   ]
                                                   [ rdf:type owl:Restriction ;
                                                     owl:onProperty :requires_sample_input ;
                                                     owl:someValuesFrom :x-ray
                                                   ]
                                                   [ rdf:type owl:Restriction ;
                                                     owl:onProperty :requires_sample_input_property ;
                                                     owl:someValuesFrom :high_pressure
                                                   ]
                                                 ) ;
                              rdf:type owl:Class
                            ] ;
        rdfs:subClassOf :experimental_technique ;
        rdfs:comment "High-Pressure X-ray Diffraction (HP-XRD) measures X-ray diffraction patterns of materials compressed to high pressures, revealing structural changes such as phase transitions, lattice compression, and equation-of-state behavior." ;
        rdfs:label "HP-XRD" ;
        <http://www.w3.org/2004/02/skos/core#prefLabel> "High-Pressure X-ray Diffraction" .


###  http://purl.org/pan-science/ESRFET#HR-XRPD
:HR-XRPD rdf:type owl:Class ;
         owl:equivalentClass [ owl:intersectionOf ( :experimental_technique
                                                    [ rdf:type owl:Restriction ;
                                                      owl:onProperty :measures_interaction_result_property ;
                                                      owl:someValuesFrom :high_precision_in_Q_space
                                                    ]
                                                    [ rdf:type owl:Restriction ;
                                                      owl:onProperty :measures_result_of_interaction ;
                                                      owl:someValuesFrom :diffraction_of_elastic_scattering
                                                    ]
                                                    [ rdf:type owl:Restriction ;
                                                      owl:onProperty :requires_sample_input ;
                                                      owl:someValuesFrom :x-ray
                                                    ]
                                                    [ rdf:type owl:Restriction ;
                                                      owl:onProperty :requires_sample_type ;
                                                      owl:someValuesFrom :powder_sample
                                                    ]
                                                  ) ;
                               rdf:type owl:Class
                             ] ;
         rdfs:comment "High-Resolution X-ray Powder Diffraction (HR-XRPD) measures diffraction patterns from powdered samples with enhanced resolution in Q-space (or d-spacing), enabling precise phase identification, accurate lattice parameter determination, and detailed structural analysis of complex materials." ;
         rdfs:label "HR-XRPD" ;
         <http://www.w3.org/2004/02/skos/core#prefLabel> "High-Resolution X-ray Powder Diffraction" .


###  http://purl.org/pan-science/ESRFET#HT-XRD
:HT-XRD rdf:type owl:Class ;
        owl:equivalentClass [ owl:intersectionOf ( :experimental_technique
                                                   [ rdf:type owl:Restriction ;
                                                     owl:onProperty :measures_result_of_interaction ;
                                                     owl:someValuesFrom :diffraction_of_elastic_scattering
                                                   ]
                                                   [ rdf:type owl:Restriction ;
                                                     owl:onProperty :requires_sample_input ;
                                                     owl:someValuesFrom :x-ray
                                                   ]
                                                   [ rdf:type owl:Restriction ;
                                                     owl:onProperty :requires_sample_input_property ;
                                                     owl:someValuesFrom :high_temperature
                                                   ]
                                                 ) ;
                              rdf:type owl:Class
                            ] ;
        rdfs:subClassOf :experimental_technique ;
        rdfs:comment "High-Temperature X-ray Diffraction (HT-XRD) measures X-ray diffraction patterns of materials at elevated temperatures, providing insights into thermal expansion, phase stability, and temperature-induced structural transformations." ;
        rdfs:label "HT-XRD" ;
        <http://www.w3.org/2004/02/skos/core#prefLabel> "High-Temperature X-ray Diffraction" .


###  http://purl.org/pan-science/ESRFET#HiP-CT
:HiP-CT rdf:type owl:Class ;
        owl:equivalentClass [ owl:intersectionOf ( :experimental_technique
                                                   [ rdf:type owl:Restriction ;
                                                     owl:onProperty :measures_as_a_function_of ;
                                                     owl:someValuesFrom :multi_sample_spatial_resolution
                                                   ]
                                                   [ rdf:type owl:Restriction ;
                                                     owl:onProperty :measures_as_a_function_of ;
                                                     owl:someValuesFrom :tomography
                                                   ]
                                                   [ rdf:type owl:Restriction ;
                                                     owl:onProperty :measures_result_of_interaction ;
                                                     owl:someValuesFrom :refraction
                                                   ]
                                                   [ rdf:type owl:Restriction ;
                                                     owl:onProperty :measures_result_of_interaction ;
                                                     owl:someValuesFrom :transmission
                                                   ]
                                                   [ rdf:type owl:Restriction ;
                                                     owl:onProperty :requires_sample_input ;
                                                     owl:someValuesFrom :x-ray
                                                   ]
                                                 ) ;
                              rdf:type owl:Class
                            ] ;
        rdfs:comment "Hierarchical Phase-Contrast Tomography (HiP-CT) measures X-ray phase-contrast projections at multiple spatial resolutions to reconstruct 3D images spanning from macroscopic to microscopic scales, enabling multiscale analysis of complex internal structures." ;
        rdfs:label "HiP-CT" ;
        <http://www.w3.org/2004/02/skos/core#prefLabel> "Hierarchical Phase-Contrast Tomography" .


###  http://purl.org/pan-science/ESRFET#IXS
:IXS rdf:type owl:Class ;
     rdfs:subClassOf :experimental_technique ;
     rdfs:comment "Inelastic X-ray Scattering (IXS) measures the energy and momentum change of X-rays scattered inelastically by a sample, providing information on electronic excitations, phonons, and other dynamic processes at the atomic scale." ;
     rdfs:label "IXS" ;
     <http://www.w3.org/2004/02/skos/core#prefLabel> "Inelastic X-ray Scattering" .


###  http://purl.org/pan-science/ESRFET#KES
:KES rdf:type owl:Class ;
     owl:equivalentClass [ owl:intersectionOf ( :experimental_technique
                                                [ rdf:type owl:Restriction ;
                                                  owl:onProperty :measures_as_a_function_of ;
                                                  owl:someValuesFrom :detection_as_a_function_of_limited_number_of_incident_energies
                                                ]
                                                [ rdf:type owl:Restriction ;
                                                  owl:onProperty :measures_as_a_function_of ;
                                                  owl:someValuesFrom <http://purl.org/pan-science/PaNET/PaNET01106>
                                                ]
                                                [ rdf:type owl:Restriction ;
                                                  owl:onProperty :measures_result_of_interaction ;
                                                  owl:someValuesFrom :transmission
                                                ]
                                              ) ;
                           rdf:type owl:Class
                         ] ;
     rdfs:comment "K-edge Subtraction Imaging (KES) measures transmitted X-ray intensity across photon energies around the absorption edge of a specific element, producing element-selective 2D maps that reveal its spatial distribution in the sample." ;
     rdfs:label "KES" ;
     <http://www.w3.org/2004/02/skos/core#prefLabel> "K-edge Subtraction Imaging" .


###  http://purl.org/pan-science/ESRFET#KESCT
:KESCT rdf:type owl:Class ;
       owl:equivalentClass [ owl:intersectionOf ( :experimental_technique
                                                  [ rdf:type owl:Restriction ;
                                                    owl:onProperty :measures_as_a_function_of ;
                                                    owl:someValuesFrom :detection_as_a_function_of_limited_number_of_incident_energies
                                                  ]
                                                  [ rdf:type owl:Restriction ;
                                                    owl:onProperty :measures_as_a_function_of ;
                                                    owl:someValuesFrom :tomography
                                                  ]
                                                  [ rdf:type owl:Restriction ;
                                                    owl:onProperty :measures_result_of_interaction ;
                                                    owl:someValuesFrom :transmission
                                                  ]
                                                  [ rdf:type owl:Restriction ;
                                                    owl:onProperty :requires_sample_input ;
                                                    owl:someValuesFrom :x-ray
                                                  ]
                                                ) ;
                             rdf:type owl:Class
                           ] ;
       rdfs:comment "K-edge Subtraction Tomography (KESCT) measures transmitted X-rays across the absorption edge of a target element at multiple projection angles to reconstruct 3D maps of elemental concentrations with high chemical specificity." ;
       rdfs:label "KESCT" ;
       <http://www.w3.org/2004/02/skos/core#prefLabel> "K-edge Subtraction Tomography" .


###  http://purl.org/pan-science/ESRFET#LDDS-XAS
:LDDS-XAS rdf:type owl:Class ;
          owl:equivalentClass [ owl:intersectionOf ( :experimental_technique
                                                     [ rdf:type owl:Restriction ;
                                                       owl:onProperty :measures_as_a_function_of ;
                                                       owl:someValuesFrom :detection_as_a_function_of_incident_energy
                                                     ]
                                                     [ rdf:type owl:Restriction ;
                                                       owl:onProperty :measures_as_a_function_of ;
                                                       owl:someValuesFrom :sample_compression
                                                     ]
                                                     [ rdf:type owl:Restriction ;
                                                       owl:onProperty :measures_interaction_result_property ;
                                                       owl:someValuesFrom :photon_count
                                                     ]
                                                     [ rdf:type owl:Restriction ;
                                                       owl:onProperty :measures_result_of_interaction ;
                                                       owl:someValuesFrom :atomic_core_excitation
                                                     ]
                                                     [ rdf:type owl:Restriction ;
                                                       owl:onProperty :requires_sample_input ;
                                                       owl:someValuesFrom :laser
                                                     ]
                                                     [ rdf:type owl:Restriction ;
                                                       owl:onProperty :requires_sample_input ;
                                                       owl:someValuesFrom :x-ray
                                                     ]
                                                   ) ;
                                rdf:type owl:Class
                              ] ;
          rdfs:comment "Laser-Driven Dynamic Compression X-ray Absorption Spectroscopy (LDDC-XAS) measures X-ray absorption spectra of materials compressed by laser-driven dynamic pressure pulses, providing time-resolved insights into electronic and structural changes under extreme conditions." ;
          rdfs:label "LDDC-XAS" ;
          <http://www.w3.org/2004/02/skos/core#prefLabel> "Laser-Driven Dynamic Compression X-ray Absorption Spectroscopy" .


###  http://purl.org/pan-science/ESRFET#LDSC-XAS
:LDSC-XAS rdf:type owl:Class ;
          owl:equivalentClass [ owl:intersectionOf ( :experimental_technique
                                                     [ rdf:type owl:Restriction ;
                                                       owl:onProperty :measures_as_a_function_of ;
                                                       owl:someValuesFrom :detection_as_a_function_of_incident_energy
                                                     ]
                                                     [ rdf:type owl:Restriction ;
                                                       owl:onProperty :measures_as_a_function_of ;
                                                       owl:someValuesFrom :shock_compression
                                                     ]
                                                     [ rdf:type owl:Restriction ;
                                                       owl:onProperty :measures_interaction_result_property ;
                                                       owl:someValuesFrom :photon_count
                                                     ]
                                                     [ rdf:type owl:Restriction ;
                                                       owl:onProperty :measures_result_of_interaction ;
                                                       owl:someValuesFrom :atomic_core_excitation
                                                     ]
                                                     [ rdf:type owl:Restriction ;
                                                       owl:onProperty :requires_sample_input ;
                                                       owl:someValuesFrom :laser
                                                     ]
                                                     [ rdf:type owl:Restriction ;
                                                       owl:onProperty :requires_sample_input ;
                                                       owl:someValuesFrom :x-ray
                                                     ]
                                                   ) ;
                                rdf:type owl:Class
                              ] ;
          rdfs:comment "Laser-Driven Shock Compression X-ray Absorption Spectroscopy (LDSC-XAS) is a specific type of Laser-Driven Dynamic Compression X-ray Absorption Spectroscopy (LDDC-XAS) that measures X-ray absorption spectra of materials subjected to laser-driven shock waves, capturing rapid structural and electronic changes during high-strain-rate compression." ;
          rdfs:label "LDSC-XAS" ;
          <http://www.w3.org/2004/02/skos/core#prefLabel> "Laser-Driven Shock Compression X-ray Absorption Spectroscopy" .


###  http://purl.org/pan-science/ESRFET#MACRO-XRF
:MACRO-XRF rdf:type owl:Class ;
           owl:equivalentClass [ owl:intersectionOf ( :experimental_technique
                                                      [ rdf:type owl:Restriction ;
                                                        owl:onProperty :measures_as_a_function_of ;
                                                        owl:someValuesFrom :macro_sample_spatial_resolution
                                                      ]
                                                      [ rdf:type owl:Restriction ;
                                                        owl:onProperty :measures_as_a_function_of ;
                                                        owl:someValuesFrom :scanning_imaging
                                                      ]
                                                      [ rdf:type owl:Restriction ;
                                                        owl:onProperty :measures_interaction_result_property ;
                                                        owl:someValuesFrom :photon_count
                                                      ]
                                                      [ rdf:type owl:Restriction ;
                                                        owl:onProperty :measures_interaction_result_property ;
                                                        owl:someValuesFrom :photon_energy
                                                      ]
                                                      [ rdf:type owl:Restriction ;
                                                        owl:onProperty :measures_result_of_interaction ;
                                                        owl:someValuesFrom :fluorescence
                                                      ]
                                                      [ rdf:type owl:Restriction ;
                                                        owl:onProperty :requires_sample_input ;
                                                        owl:someValuesFrom :x-ray
                                                      ]
                                                    ) ;
                                 rdf:type owl:Class
                               ] ;
           rdfs:comment "XRF which provides elemental distributions in a 2D projection of the sample in space. The spatial separation is achieved by moving the sample through a beam is beam size greater that 100 micron." ;
           rdfs:label "MACRO-XRF" ;
           <http://www.w3.org/2004/02/skos/core#altLabel> "MA-XRF" ,
                                                          "Macro-XRF" ;
           <http://www.w3.org/2004/02/skos/core#prefLabel> "Scanning Macro X-ray fluorescence" .


###  http://purl.org/pan-science/ESRFET#MAD
:MAD rdf:type owl:Class ;
     rdfs:subClassOf :experimental_technique ;
     rdfs:comment "Multi-wavelength Anomalous Dispersion (MAD) measures diffraction at multiple X-ray wavelengths around an absorption edge to use anomalous scattering differences for more accurate phase determination in crystallography." ;
     rdfs:label "MAD" ;
     <http://www.w3.org/2004/02/skos/core#prefLabel> "Multi-wavelength Anomalous Dispersion" .


###  http://purl.org/pan-science/ESRFET#MBS
:MBS rdf:type owl:Class ;
     rdfs:subClassOf :experimental_technique ;
     rdfs:comment "Mössbauer spectroscopy measures the resonant absorption of X-rays by atomic nuclei in a solid to derive information on oxidation state, magnetic properties, and local chemical environment of Mössbauer-active isotopes (e.g. Fe-57)." ;
     rdfs:label "MBS" ;
     <http://www.w3.org/2004/02/skos/core#prefLabel> "Mössbauer Spectroscopy" .


###  http://purl.org/pan-science/ESRFET#MICRO-XRD
:MICRO-XRD rdf:type owl:Class ;
           owl:equivalentClass [ owl:intersectionOf ( :experimental_technique
                                                      [ rdf:type owl:Restriction ;
                                                        owl:onProperty :measures_as_a_function_of ;
                                                        owl:someValuesFrom :micro_sample_spatial_resolution
                                                      ]
                                                      [ rdf:type owl:Restriction ;
                                                        owl:onProperty :measures_as_a_function_of ;
                                                        owl:someValuesFrom :scanning_imaging
                                                      ]
                                                      [ rdf:type owl:Restriction ;
                                                        owl:onProperty :measures_result_of_interaction ;
                                                        owl:someValuesFrom :diffraction_of_elastic_scattering
                                                      ]
                                                      [ rdf:type owl:Restriction ;
                                                        owl:onProperty :requires_sample_input ;
                                                        owl:someValuesFrom :x-ray
                                                      ]
                                                    ) ;
                                 rdf:type owl:Class
                               ] ;
           rdfs:comment "XRD which provides small-scale feature or phase distributions in a 2D projection of the sample in space. The spatial separation is achieved by moving the sample through a beam is beam size between 0.1 and 100 micron." ;
           rdfs:label "MICRO-XRD" ;
           <http://www.w3.org/2004/02/skos/core#altLabel> "Micro-XRD" ,
                                                          "μ-XRD" ;
           <http://www.w3.org/2004/02/skos/core#prefLabel> "Scanning Micro X-ray diffraction" .


###  http://purl.org/pan-science/ESRFET#MICRO-XRF
:MICRO-XRF rdf:type owl:Class ;
           owl:equivalentClass [ owl:intersectionOf ( :experimental_technique
                                                      [ rdf:type owl:Restriction ;
                                                        owl:onProperty :measures_as_a_function_of ;
                                                        owl:someValuesFrom :micro_sample_spatial_resolution
                                                      ]
                                                      [ rdf:type owl:Restriction ;
                                                        owl:onProperty :measures_as_a_function_of ;
                                                        owl:someValuesFrom :scanning_imaging
                                                      ]
                                                      [ rdf:type owl:Restriction ;
                                                        owl:onProperty :measures_interaction_result_property ;
                                                        owl:someValuesFrom :photon_count
                                                      ]
                                                      [ rdf:type owl:Restriction ;
                                                        owl:onProperty :measures_interaction_result_property ;
                                                        owl:someValuesFrom :photon_energy
                                                      ]
                                                      [ rdf:type owl:Restriction ;
                                                        owl:onProperty :measures_result_of_interaction ;
                                                        owl:someValuesFrom :fluorescence
                                                      ]
                                                      [ rdf:type owl:Restriction ;
                                                        owl:onProperty :requires_sample_input ;
                                                        owl:someValuesFrom :x-ray
                                                      ]
                                                    ) ;
                                 rdf:type owl:Class
                               ] ;
           rdfs:comment "XRF which provides elemental distributions in a 2D projection of the sample in space. The spatial separation is achieved by moving the sample through a beam is beam size between 0.1 and 100 micron." ;
           rdfs:label "MICRO-XRF" ;
           <http://www.w3.org/2004/02/skos/core#altLabel> "Micro-XRF" ,
                                                          "μ-XRF" ;
           <http://www.w3.org/2004/02/skos/core#prefLabel> "Scanning Micro X-ray fluorescence" .


###  http://purl.org/pan-science/ESRFET#MPES
:MPES rdf:type owl:Class ;
      rdfs:subClassOf :experimental_technique ;
      rdfs:comment "Momentum-Resolved Photoemission Spectroscopy (MPES) measures electron emission as a function of momentum and energy to reveal the dispersion and symmetry of electronic states in solids." ;
      rdfs:label "MPES" ;
      <http://www.w3.org/2004/02/skos/core#prefLabel> "Momentum-Resolved Photoemission Spectroscopy" .


###  http://purl.org/pan-science/ESRFET#MRT
:MRT rdf:type owl:Class ;
     rdfs:subClassOf :experimental_technique ;
     rdfs:comment "Microbeam Radiation Therapy (MRT) uses arrays of microscale, high-dose X-ray beams to irradiate tissue with high spatial precision, aiming to maximize tumor damage while sparing surrounding healthy tissue." ;
     rdfs:label "MRT" ;
     <http://www.w3.org/2004/02/skos/core#prefLabel> "Microbeam Radiation Therapy" .


###  http://purl.org/pan-science/ESRFET#MX
:MX rdf:type owl:Class ;
    rdfs:subClassOf :experimental_technique ;
    rdfs:comment "Macromolecular Crystallography (MX) measures X-ray diffraction from crystals of biological macromolecules to determine their 3D atomic structures, providing insights into protein folding, function, and interactions." ;
    rdfs:label "MX" ;
    <http://www.w3.org/2004/02/skos/core#prefLabel> "Macromolecular Crystallography" .


###  http://purl.org/pan-science/ESRFET#NANO-XRD
:NANO-XRD rdf:type owl:Class ;
          owl:equivalentClass [ owl:intersectionOf ( :experimental_technique
                                                     [ rdf:type owl:Restriction ;
                                                       owl:onProperty :measures_as_a_function_of ;
                                                       owl:someValuesFrom :nano_sample_spatial_resolution
                                                     ]
                                                     [ rdf:type owl:Restriction ;
                                                       owl:onProperty :measures_as_a_function_of ;
                                                       owl:someValuesFrom :scanning_imaging
                                                     ]
                                                     [ rdf:type owl:Restriction ;
                                                       owl:onProperty :measures_result_of_interaction ;
                                                       owl:someValuesFrom :diffraction_of_elastic_scattering
                                                     ]
                                                     [ rdf:type owl:Restriction ;
                                                       owl:onProperty :requires_sample_input ;
                                                       owl:someValuesFrom :x-ray
                                                     ]
                                                   ) ;
                                rdf:type owl:Class
                              ] ;
          rdfs:comment "XRD which provides small-scale feature or phase distributions in a 2D projection of the sample in space. The spatial separation is achieved by moving the sample through a beam is beam size between 0.1 and 100 nanometers." ;
          rdfs:label "NANO-XRD" ;
          <http://www.w3.org/2004/02/skos/core#altLabel> "Nano-XRD" ,
                                                         "nXRD" ;
          <http://www.w3.org/2004/02/skos/core#prefLabel> "Scanning Nano X-ray diffraction" .


###  http://purl.org/pan-science/ESRFET#NANO-XRF
:NANO-XRF rdf:type owl:Class ;
          owl:equivalentClass [ owl:intersectionOf ( :experimental_technique
                                                     [ rdf:type owl:Restriction ;
                                                       owl:onProperty :measures_as_a_function_of ;
                                                       owl:someValuesFrom :nano_sample_spatial_resolution
                                                     ]
                                                     [ rdf:type owl:Restriction ;
                                                       owl:onProperty :measures_as_a_function_of ;
                                                       owl:someValuesFrom :scanning_imaging
                                                     ]
                                                     [ rdf:type owl:Restriction ;
                                                       owl:onProperty :measures_interaction_result_property ;
                                                       owl:someValuesFrom :photon_count
                                                     ]
                                                     [ rdf:type owl:Restriction ;
                                                       owl:onProperty :measures_interaction_result_property ;
                                                       owl:someValuesFrom :photon_energy
                                                     ]
                                                     [ rdf:type owl:Restriction ;
                                                       owl:onProperty :measures_result_of_interaction ;
                                                       owl:someValuesFrom :fluorescence
                                                     ]
                                                     [ rdf:type owl:Restriction ;
                                                       owl:onProperty :requires_sample_input ;
                                                       owl:someValuesFrom :x-ray
                                                     ]
                                                   ) ;
                                rdf:type owl:Class
                              ] ;
          rdfs:comment "XRF which provides elemental distributions in a 2D projection of the sample in space. The spatial separation is achieved by moving the sample through a beam is beam size between 0.1 and 100 nanometers." ;
          rdfs:label "NANO-XRF" ;
          <http://www.w3.org/2004/02/skos/core#altLabel> "Nano-XRF" ,
                                                         "n-XRF" ;
          <http://www.w3.org/2004/02/skos/core#prefLabel> "Scanning Nano X-ray fluorescence" .


###  http://purl.org/pan-science/ESRFET#NFP
:NFP rdf:type owl:Class ;
     rdfs:subClassOf :experimental_technique ;
     rdfs:comment "Near-Field Ptychography (NFP) measures coherent diffraction patterns collected in the near-field regime by scanning overlapping illumination spots, enabling high-resolution phase and amplitude imaging of samples." ;
     rdfs:label "NFP" ;
     <http://www.w3.org/2004/02/skos/core#prefLabel> "Near-Field Ptychography" .


###  http://purl.org/pan-science/ESRFET#NFS
:NFS rdf:type owl:Class ;
     rdfs:subClassOf :experimental_technique ;
     rdfs:comment "Nuclear Forward Scattering (NFS) measures the time-resolved resonant scattering of synchrotron-generated X-rays in the forward direction, extracting hyperfine parameters (e.g. isomer shift, quadrupole splitting, magnetic splitting) from the temporal interference pattern." ,
                  "Time-domain analog of Mössbauer spectroscopy" ;
     rdfs:label "NFS" ;
     <http://www.w3.org/2004/02/skos/core#prefLabel> "Nuclear Forward Scattering" .


###  http://purl.org/pan-science/ESRFET#NR-XMLD
:NR-XMLD rdf:type owl:Class ;
         rdfs:subClassOf :experimental_technique ;
         rdfs:comment "Non-Reciprocal X-ray Magnetic Linear Dichroism (NR-XMLD) measures differences in linear X-ray absorption depending on magnetization direction and X-ray polarization, revealing magnetic asymmetries that break time-reversal symmetry." ;
         rdfs:label "NR-XMLD" ;
         <http://www.w3.org/2004/02/skos/core#prefLabel> "Non-Reciprocal X-ray Magnetic Linear Dichroism" .


###  http://purl.org/pan-science/ESRFET#NRIXS
:NRIXS rdf:type owl:Class ;
       rdfs:subClassOf :experimental_technique ;
       rdfs:comment "Nuclear Resonant Inelastic X-ray Scattering (NRIXS) measures the energy distribution of X-rays scattered inelastically by nuclear resonances, providing element-specific information on phonon density of states and lattice dynamics." ;
       rdfs:label "NRIXS" ;
       <http://www.w3.org/2004/02/skos/core#prefLabel> "Nuclear Resonant Inelastic X-ray Scattering" .


###  http://purl.org/pan-science/ESRFET#NRS
:NRS rdf:type owl:Class ;
     rdfs:subClassOf :experimental_technique ;
     rdfs:comment "Nuclear Resonant Scattering (NRS) measures time-delayed resonant scattering of X-rays from Mössbauer-active nuclei to study hyperfine interactions, magnetic order, and dynamics at the atomic scale." ;
     rdfs:label "NRS" ;
     <http://www.w3.org/2004/02/skos/core#prefLabel> "Nuclear Resonant Scattering" .


###  http://purl.org/pan-science/ESRFET#PB-XPCI
:PB-XPCI rdf:type owl:Class ;
         owl:equivalentClass [ owl:intersectionOf ( :experimental_technique
                                                    [ rdf:type owl:Restriction ;
                                                      owl:onProperty :measures_as_a_function_of ;
                                                      owl:someValuesFrom <http://purl.org/pan-science/PaNET/PaNET01106>
                                                    ]
                                                    [ rdf:type owl:Restriction ;
                                                      owl:onProperty :measures_result_of_interaction ;
                                                      owl:someValuesFrom :refraction
                                                    ]
                                                    [ rdf:type owl:Restriction ;
                                                      owl:onProperty :measures_result_of_interaction ;
                                                      owl:someValuesFrom :transmission
                                                    ]
                                                    [ rdf:type owl:Restriction ;
                                                      owl:onProperty :requires_sample_input ;
                                                      owl:someValuesFrom :x-ray
                                                    ]
                                                    [ rdf:type owl:Restriction ;
                                                      owl:onProperty :requires_sample_input_property ;
                                                      owl:someValuesFrom :unmodified_beam
                                                    ]
                                                  ) ;
                               rdf:type owl:Class
                             ] ;
         rdfs:comment "Propagation-Based X-ray Phase-Contrast Imaging (PB-XPCI) measures phase-induced interference fringes that form as X-rays propagate beyond a sample, producing 2D images with enhanced contrast for weakly absorbing or low-Z materials. By placing the detector at a sufficient distance from the sample, PB-XPCI converts subtle phase variations into measurable intensity modulations, revealing fine internal features and interfaces not visible in conventional absorption imaging." ;
         rdfs:label "PB-XPCI" ;
         <http://www.w3.org/2004/02/skos/core#prefLabel> "Propagation-Based X-ray Phase-Contrast Imaging" .


###  http://purl.org/pan-science/ESRFET#PB-XPCT
:PB-XPCT rdf:type owl:Class ;
         owl:equivalentClass [ owl:intersectionOf ( :experimental_technique
                                                    [ rdf:type owl:Restriction ;
                                                      owl:onProperty :measures_as_a_function_of ;
                                                      owl:someValuesFrom :tomography
                                                    ]
                                                    [ rdf:type owl:Restriction ;
                                                      owl:onProperty :measures_result_of_interaction ;
                                                      owl:someValuesFrom :refraction
                                                    ]
                                                    [ rdf:type owl:Restriction ;
                                                      owl:onProperty :measures_result_of_interaction ;
                                                      owl:someValuesFrom :transmission
                                                    ]
                                                    [ rdf:type owl:Restriction ;
                                                      owl:onProperty :requires_sample_input ;
                                                      owl:someValuesFrom :x-ray
                                                    ]
                                                    [ rdf:type owl:Restriction ;
                                                      owl:onProperty :requires_sample_input_property ;
                                                      owl:someValuesFrom :unmodified_beam
                                                    ]
                                                  ) ;
                               rdf:type owl:Class
                             ] ;
         rdfs:comment "X-ray Propagation Phase-Contrast Tomography (PB-XPCT) measures phase-induced interference patterns that form as X-rays propagate beyond the sample, reconstructing 3D phase-contrast images by recording projections at sufficient sample–detector distances." ;
         rdfs:label "PB-XPCT" ;
         <http://www.w3.org/2004/02/skos/core#prefLabel> "Propagation-based X-ray Phase-Contrast Tomograph" .


###  http://purl.org/pan-science/ESRFET#PCI
:PCI rdf:type owl:Class ;
     owl:equivalentClass [ owl:intersectionOf ( :experimental_technique
                                                [ rdf:type owl:Restriction ;
                                                  owl:onProperty :measures_as_a_function_of ;
                                                  owl:someValuesFrom <http://purl.org/pan-science/PaNET/PaNET01106>
                                                ]
                                                [ rdf:type owl:Restriction ;
                                                  owl:onProperty :measures_result_of_interaction ;
                                                  owl:someValuesFrom :refraction
                                                ]
                                                [ rdf:type owl:Restriction ;
                                                  owl:onProperty :requires_sample_input ;
                                                  owl:someValuesFrom :x-ray
                                                ]
                                              ) ;
                           rdf:type owl:Class
                         ] ;
     rdfs:comment "Phase-Contrast X-ray Imaging (PCI) measures phase shifts of X-rays transmitted through a sample to generate 2D images with enhanced contrast for weakly absorbing or low-Z materials. By exploiting phase variations rather than absorption, PCI reveals fine structural details such as internal boundaries, fibers, and low-density regions that are invisible in conventional absorption-based X-ray imaging." ;
     rdfs:label "PCI" ;
     <http://www.w3.org/2004/02/skos/core#prefLabel> "Phase-Contrast X-ray Imaging" .


###  http://purl.org/pan-science/ESRFET#PDF
:PDF rdf:type owl:Class ;
     rdfs:subClassOf :experimental_technique ;
     rdfs:comment "Pair Distribution Function (PDF) analysis measures the distribution of interatomic distances by Fourier-transforming total scattering data, revealing local atomic arrangements and disorder in both crystalline and amorphous materials." ;
     rdfs:label "PDF" ;
     <http://www.w3.org/2004/02/skos/core#prefLabel> "Pair Distribution Function" .


###  http://purl.org/pan-science/ESRFET#PFY-XAS
:PFY-XAS rdf:type owl:Class ;
         owl:equivalentClass [ owl:intersectionOf ( :experimental_technique
                                                    [ rdf:type owl:Restriction ;
                                                      owl:onProperty :measures_as_a_function_of ;
                                                      owl:someValuesFrom :detection_as_a_function_of_incident_energy
                                                    ]
                                                    [ rdf:type owl:Restriction ;
                                                      owl:onProperty :measures_interaction_result_property ;
                                                      owl:someValuesFrom :photon_count
                                                    ]
                                                    [ rdf:type owl:Restriction ;
                                                      owl:onProperty :measures_result_of_interaction ;
                                                      owl:someValuesFrom :atomic_core_excitation
                                                    ]
                                                    [ rdf:type owl:Restriction ;
                                                      owl:onProperty :measures_result_of_interaction ;
                                                      owl:someValuesFrom :fluorescence
                                                    ]
                                                    [ rdf:type owl:Restriction ;
                                                      owl:onProperty :requires_sample_input ;
                                                      owl:someValuesFrom :x-ray
                                                    ]
                                                  ) ;
                               rdf:type owl:Class
                             ] ;
         rdfs:comment "Partial Fluorescence Yield X-ray Absorption Spectroscopy (PFY-XAS) measures fluorescence photons from specific emission lines as a function of incident X-ray energy, providing element- and site-selective absorption spectra with reduced self-absorption effects." ;
         rdfs:label "PFY-XAS" ;
         <http://www.w3.org/2004/02/skos/core#prefLabel> "Partial Fluorescence Yield X-ray Absorption Spectroscopy" .


###  http://purl.org/pan-science/ESRFET#PIXE
:PIXE rdf:type owl:Class ;
      owl:equivalentClass [ owl:intersectionOf ( :experimental_technique
                                                 [ rdf:type owl:Restriction ;
                                                   owl:onProperty :measures_interaction_result_property ;
                                                   owl:someValuesFrom :photon_count
                                                 ]
                                                 [ rdf:type owl:Restriction ;
                                                   owl:onProperty :measures_interaction_result_property ;
                                                   owl:someValuesFrom :photon_energy
                                                 ]
                                                 [ rdf:type owl:Restriction ;
                                                   owl:onProperty :measures_result_of_interaction ;
                                                   owl:someValuesFrom :fluorescence
                                                 ]
                                                 [ rdf:type owl:Restriction ;
                                                   owl:onProperty :requires_sample_input ;
                                                   owl:someValuesFrom :charged_particles
                                                 ]
                                               ) ;
                            rdf:type owl:Class
                          ] ;
      rdfs:comment "Particle Induced X-ray Emission (PIXE) measures characteristic X-rays emitted by a sample when irradiated with energetic charged particles (e.g., protons) to determine elemental composition with high sensitivity." ;
      rdfs:label "PIXE" ;
      <http://www.w3.org/2004/02/skos/core#prefLabel> "Particle Induced X-ray Emission" .


###  http://purl.org/pan-science/ESRFET#PTYCHO
:PTYCHO rdf:type owl:Class ;
        rdfs:subClassOf :experimental_technique ;
        rdfs:comment "Ptychography (PTYCHO) measures coherent diffraction patterns by scanning overlapping illumination spots on a sample in the far field, reconstructing high-resolution complex-valued images of sample structure beyond conventional lens limitations." ;
        rdfs:label "PTYCHO" ;
        <http://www.w3.org/2004/02/skos/core#prefLabel> "Ptychography" .


###  http://purl.org/pan-science/ESRFET#PXCT
:PXCT rdf:type owl:Class ;
      rdfs:subClassOf :experimental_technique ;
      rdfs:comment "Ptychographic X-ray Computed Tomography (PXCT) combines coherent diffraction imaging and tomography by scanning overlapping regions at multiple angles to reconstruct 3D quantitative electron density maps with nanometer-scale resolution." ;
      rdfs:label "PXCT" ;
      <http://www.w3.org/2004/02/skos/core#prefLabel> "Ptychographic X-ray Computed Tomography" .


###  http://purl.org/pan-science/ESRFET#REXS
:REXS rdf:type owl:Class ;
      rdfs:subClassOf :experimental_technique ;
      rdfs:comment "Resonant Elastic X-ray Scattering (REXS) measures elastic scattering near an absorption edge to enhance contrast from specific elements, revealing electronic, magnetic, and orbital ordering in materials." ;
      rdfs:label "REXS" ;
      <http://www.w3.org/2004/02/skos/core#prefLabel> "Resonant Elastic X-ray Scattering" .


###  http://purl.org/pan-science/ESRFET#RIXS
:RIXS rdf:type owl:Class ;
      rdfs:subClassOf :experimental_technique ;
      rdfs:comment "Resonant Inelastic X-ray Scattering (RIXS) measures energy loss of X-rays scattered resonantly from a sample, providing detailed insights into electronic excitations, spin dynamics, and valence states." ;
      rdfs:label "RIXS" ;
      <http://www.w3.org/2004/02/skos/core#prefLabel> "Resonant Inelastic X-ray Scattering" .


###  http://purl.org/pan-science/ESRFET#RXES
:RXES rdf:type owl:Class ;
      rdfs:subClassOf :experimental_technique ;
      rdfs:comment "Resonant X-ray Emission Spectroscopy (RXES) measures emitted X-rays following resonant excitation of core electrons, providing element- and valence-specific information about electronic structure and chemical states." ;
      rdfs:label "RXES" ;
      <http://www.w3.org/2004/02/skos/core#prefLabel> "Resonant X-ray Emission Spectroscopy" .


###  http://purl.org/pan-science/ESRFET#S-XRD
:S-XRD rdf:type owl:Class ;
       owl:equivalentClass [ owl:intersectionOf ( :experimental_technique
                                                  [ rdf:type owl:Restriction ;
                                                    owl:onProperty :measures_as_a_function_of ;
                                                    owl:someValuesFrom :scanning_imaging
                                                  ]
                                                  [ rdf:type owl:Restriction ;
                                                    owl:onProperty :measures_result_of_interaction ;
                                                    owl:someValuesFrom :diffraction_of_elastic_scattering
                                                  ]
                                                  [ rdf:type owl:Restriction ;
                                                    owl:onProperty :requires_sample_input ;
                                                    owl:someValuesFrom :x-ray
                                                  ]
                                                ) ;
                             rdf:type owl:Class
                           ] ;
       rdfs:subClassOf :experimental_technique ;
       rdfs:comment "Scanning X-ray Diffraction (S-XRD) measures diffraction patterns at many scanned positions on a sample using a focused X-ray beam, providing spatially resolved 2D maps of crystal structure, phase distribution, and strain within the sample." ;
       rdfs:label "S-XRD" ;
       <http://www.w3.org/2004/02/skos/core#altLabel> "SXDM" ,
                                                      "SXRD" ,
                                                      "Scanning X-ray Diffraction Microscopy" ;
       <http://www.w3.org/2004/02/skos/core#prefLabel> "Scanning X-ray Diffraction" .


###  http://purl.org/pan-science/ESRFET#S-XRF
:S-XRF rdf:type owl:Class ;
       owl:equivalentClass [ owl:intersectionOf ( :experimental_technique
                                                  [ rdf:type owl:Restriction ;
                                                    owl:onProperty :measures_as_a_function_of ;
                                                    owl:someValuesFrom :scanning_imaging
                                                  ]
                                                  [ rdf:type owl:Restriction ;
                                                    owl:onProperty :measures_interaction_result_property ;
                                                    owl:someValuesFrom :photon_count
                                                  ]
                                                  [ rdf:type owl:Restriction ;
                                                    owl:onProperty :measures_interaction_result_property ;
                                                    owl:someValuesFrom :photon_energy
                                                  ]
                                                  [ rdf:type owl:Restriction ;
                                                    owl:onProperty :measures_result_of_interaction ;
                                                    owl:someValuesFrom :fluorescence
                                                  ]
                                                  [ rdf:type owl:Restriction ;
                                                    owl:onProperty :requires_sample_input ;
                                                    owl:someValuesFrom :x-ray
                                                  ]
                                                ) ;
                             rdf:type owl:Class
                           ] ;
       rdfs:comment "Scanning X-ray Fluorescence (S-XRF) measures elemental composition by scanning a focused X-ray beam across a sample and detecting emitted fluorescence, producing high-resolution 2D maps of elemental distributions in the sample." ;
       rdfs:label "S-XRF" ;
       <http://www.w3.org/2004/02/skos/core#prefLabel> "Scanning X-ray Fluorescence" .


###  http://purl.org/pan-science/ESRFET#SAD
:SAD rdf:type owl:Class ;
     rdfs:subClassOf :experimental_technique ;
     rdfs:comment "Single-wavelength Anomalous Diffraction (SAD) measures diffraction at one specific X-ray wavelength near an absorption edge to exploit anomalous scattering for phase determination in crystallography." ;
     rdfs:label "SAD" ;
     <http://www.w3.org/2004/02/skos/core#prefLabel> "Single-wavelength Anomalous Diffraction" .


###  http://purl.org/pan-science/ESRFET#SAXS
:SAXS rdf:type owl:Class ;
      owl:equivalentClass [ owl:intersectionOf ( :experimental_technique
                                                 [ rdf:type owl:Restriction ;
                                                   owl:onProperty :measures_interaction_result_property ;
                                                   owl:someValuesFrom :large_length_scales
                                                 ]
                                                 [ rdf:type owl:Restriction ;
                                                   owl:onProperty :measures_result_of_interaction ;
                                                   owl:someValuesFrom :diffraction_of_elastic_scattering
                                                 ]
                                                 [ rdf:type owl:Restriction ;
                                                   owl:onProperty :requires_sample_input ;
                                                   owl:someValuesFrom :x-ray
                                                 ]
                                               ) ;
                            rdf:type owl:Class
                          ] ;
      rdfs:comment "Small-Angle X-ray Scattering (SAXS) measures the X-ray scattering intensity at small angles to obtain information about the size, shape, and structural organization of nanoscale features in a sample." ;
      rdfs:label "SAXS" ;
      <http://www.w3.org/2004/02/skos/core#prefLabel> "Small-Angle X-ray Scattering" .


###  http://purl.org/pan-science/ESRFET#SCXRD
:SCXRD rdf:type owl:Class ;
       owl:equivalentClass [ owl:intersectionOf ( :experimental_technique
                                                  [ rdf:type owl:Restriction ;
                                                    owl:onProperty :measures_result_of_interaction ;
                                                    owl:someValuesFrom :diffraction_of_elastic_scattering
                                                  ]
                                                  [ rdf:type owl:Restriction ;
                                                    owl:onProperty :requires_sample_input ;
                                                    owl:someValuesFrom :x-ray
                                                  ]
                                                  [ rdf:type owl:Restriction ;
                                                    owl:onProperty :requires_sample_type ;
                                                    owl:someValuesFrom :single_crystal_sample
                                                  ]
                                                ) ;
                             rdf:type owl:Class
                           ] ;
       rdfs:comment "Single Crystal X-ray Diffraction (SCXRD) measures X-ray diffraction from a single crystal to determine its precise 3D crystal structure, including atomic positions, bonding, and symmetry." ;
       rdfs:label "SCXRD" ;
       <http://www.w3.org/2004/02/skos/core#altLabel> "SC-XRD" ,
                                                      "SCD" ,
                                                      "SXRD" ;
       <http://www.w3.org/2004/02/skos/core#prefLabel> "Single Crystal X-ray Diffraction" .


###  http://purl.org/pan-science/ESRFET#SIXES
:SIXES rdf:type owl:Class ;
       owl:equivalentClass [ owl:intersectionOf ( :experimental_technique
                                                  [ rdf:type owl:Restriction ;
                                                    owl:onProperty :measures_as_a_function_of ;
                                                    owl:someValuesFrom :detection_as_a_function_of_limited_number_of_incident_energies
                                                  ]
                                                  [ rdf:type owl:Restriction ;
                                                    owl:onProperty :measures_as_a_function_of ;
                                                    owl:someValuesFrom :scanning_imaging
                                                  ]
                                                  [ rdf:type owl:Restriction ;
                                                    owl:onProperty :measures_interaction_result_property ;
                                                    owl:someValuesFrom :photon_count
                                                  ]
                                                  [ rdf:type owl:Restriction ;
                                                    owl:onProperty :measures_interaction_result_property ;
                                                    owl:someValuesFrom :photon_energy
                                                  ]
                                                  [ rdf:type owl:Restriction ;
                                                    owl:onProperty :measures_result_of_interaction ;
                                                    owl:someValuesFrom :atomic_core_excitation
                                                  ]
                                                  [ rdf:type owl:Restriction ;
                                                    owl:onProperty :measures_result_of_interaction ;
                                                    owl:someValuesFrom :fluorescence
                                                  ]
                                                  [ rdf:type owl:Restriction ;
                                                    owl:onProperty :requires_sample_input ;
                                                    owl:someValuesFrom :x-ray
                                                  ]
                                                ) ;
                             rdf:type owl:Class
                           ] ;
       rdfs:comment "Selectively Induced X-ray Emission Spectroscopy (SIXES) measures element- and state-specific X-ray emission by selectively exciting particular electronic states, recording a limited number of scanning X-ray fluorescence (S-XRF) maps at selected incident energies. This approach provides detailed insights into the electronic structure and chemical environment of complex materials while reducing data volume compared to full XANES mapping." ,
                    """Two definitions seem to exist for SIXES:
Sakurai et. al. (1988): XAS with a Si(Li) detector.
Simionovici et al (2000): XRF maps at a few incident energies.
The second definition is chosen for this technique.""" ;
       rdfs:label "SIXES" ;
       <http://www.w3.org/2004/02/skos/core#prefLabel> "Selectively Induced X-ray Emission Spectroscopy" .


###  http://purl.org/pan-science/ESRFET#SMS
:SMS rdf:type owl:Class ;
     rdfs:subClassOf :experimental_technique ;
     rdfs:comment "The Synchrotron Mössbauer Source (SMS) provides a highly collimated, monochromatic beam of resonant X-rays (e.g. 14.4 keV for Fe-57), enabling Mössbauer spectroscopy with high spatial resolution, fast time resolution, and compatibility with micro- and nano-focused X-ray techniques." ;
     rdfs:label "SMS" ;
     <http://www.w3.org/2004/02/skos/core#prefLabel> "Synchrotron Mössbauer Spectroscopy" .


###  http://purl.org/pan-science/ESRFET#SMX
:SMX rdf:type owl:Class ;
     rdfs:subClassOf :experimental_technique ;
     rdfs:comment "Serial Macromolecular Crystallography (SMX) is a subset of SSX focused on collecting diffraction data from many small macromolecular crystals, allowing high-resolution structural analysis of proteins and complexes that are challenging to crystallize." ;
     rdfs:label "SMX" ;
     <http://www.w3.org/2004/02/skos/core#prefLabel> "Serial Macromolecular Crystallography" .


###  http://purl.org/pan-science/ESRFET#SSX
:SSX rdf:type owl:Class ;
     owl:equivalentClass [ owl:intersectionOf ( :experimental_technique
                                                [ rdf:type owl:Restriction ;
                                                  owl:onProperty :measures_as_a_function_of ;
                                                  owl:someValuesFrom :serial_screening
                                                ]
                                                [ rdf:type owl:Restriction ;
                                                  owl:onProperty :measures_result_of_interaction ;
                                                  owl:someValuesFrom :diffraction_of_elastic_scattering
                                                ]
                                                [ rdf:type owl:Restriction ;
                                                  owl:onProperty :requires_sample_input ;
                                                  owl:someValuesFrom :x-ray
                                                ]
                                              ) ;
                           rdf:type owl:Class
                         ] ;
     rdfs:comment "Serial Synchrotron Crystallography (SSX) is similar to Single Crystal X-ray Diffraction (SCXRD), but instead of measuring diffraction from one crystal in multiple orientations, SSX collects diffraction from many micro- or nano-crystals with random orientations sequentially at a synchrotron, enabling structure determination from samples that cannot grow large single crystals." ;
     rdfs:label "SSX" ;
     <http://www.w3.org/2004/02/skos/core#prefLabel> "Serial Synchrotron Crystallography" .


###  http://purl.org/pan-science/ESRFET#STXM
:STXM rdf:type owl:Class ;
      rdfs:subClassOf :experimental_technique ;
      rdfs:comment "Scanning Transmission X-ray Microscopy (STXM) measures X-ray transmission through a sample by scanning a focused X-ray beam in 2D, providing spatially resolved chemical, elemental, and morphological maps at nanometer-scale resolution." ;
      rdfs:label "STXM" ;
      <http://www.w3.org/2004/02/skos/core#prefLabel> "Scanning Transmission X-ray Microscopy" .


###  http://purl.org/pan-science/ESRFET#TEM
:TEM rdf:type owl:Class ;
     owl:equivalentClass [ owl:intersectionOf ( :experimental_technique
                                                [ rdf:type owl:Restriction ;
                                                  owl:onProperty :measures_result_of_interaction ;
                                                  owl:someValuesFrom :transmission
                                                ]
                                                [ rdf:type owl:Restriction ;
                                                  owl:onProperty :requires_sample_input ;
                                                  owl:someValuesFrom :electrons
                                                ]
                                              ) ;
                           rdf:type owl:Class
                         ] ;
     rdfs:comment "Transmission Electron Microscopy (TEM) measures electrons transmitted through an ultra-thin sample to produce high-resolution images of its internal structure, enabling atomic- to nanometer-scale imaging and analysis of morphology, crystallography, and defects." ;
     rdfs:label "TEM" ;
     <http://www.w3.org/2004/02/skos/core#prefLabel> "Transmission Electron Microscopy" .


###  http://purl.org/pan-science/ESRFET#TFY-XAS
:TFY-XAS rdf:type owl:Class ;
         owl:equivalentClass [ owl:intersectionOf ( :experimental_technique
                                                    [ rdf:type owl:Restriction ;
                                                      owl:onProperty :measures_as_a_function_of ;
                                                      owl:someValuesFrom :detection_as_a_function_of_incident_energy
                                                    ]
                                                    [ rdf:type owl:Restriction ;
                                                      owl:onProperty :measures_interaction_result_property ;
                                                      owl:someValuesFrom :photon_count
                                                    ]
                                                    [ rdf:type owl:Restriction ;
                                                      owl:onProperty :measures_result_of_interaction ;
                                                      owl:someValuesFrom :atomic_core_excitation
                                                    ]
                                                    [ rdf:type owl:Restriction ;
                                                      owl:onProperty :measures_result_of_interaction ;
                                                      owl:someValuesFrom :fluorescence
                                                    ]
                                                    [ rdf:type owl:Restriction ;
                                                      owl:onProperty :requires_sample_input ;
                                                      owl:someValuesFrom :x-ray
                                                    ]
                                                  ) ;
                               rdf:type owl:Class
                             ] ;
         rdfs:comment "Total Fluorescence Yield X-ray Absorption Spectroscopy (TFY-XAS) measures the total emitted fluorescence photons as a function of incident X-ray energy to determine element-specific absorption spectra, providing bulk-sensitive information about electronic and structural properties." ;
         rdfs:label "TFY-XAS" ;
         <http://www.w3.org/2004/02/skos/core#prefLabel> "Total Fluorescence Yield X-ray Absorption Spectroscopy" .


###  http://purl.org/pan-science/ESRFET#TR-MX
:TR-MX rdf:type owl:Class ;
       rdfs:subClassOf :experimental_technique ;
       rdfs:comment "Time-Resolved Macromolecular Crystallography (TR-MX) measures X-ray diffraction from macromolecular crystals at successive time points following a reaction trigger (e.g., laser pulse or substrate injection), enabling the observation of structural changes in biomolecules during a reaction or functional cycle." ;
       rdfs:label "TR-MX" ;
       <http://www.w3.org/2004/02/skos/core#prefLabel> "Time-Resolved Macromolecular Crystallography" .


###  http://purl.org/pan-science/ESRFET#TR-USAXS
:TR-USAXS rdf:type owl:Class ;
          rdfs:subClassOf :experimental_technique ;
          rdfs:comment "Time-Resolved Ultra-Small Angle X-ray Scattering (TR-USAXS) measures ultra-small angle X-ray scattering as a function of time to monitor structural evolution and dynamics of large-scale features such as aggregation, phase separation, or self-assembly." ;
          rdfs:label "TR-USAXS" ;
          <http://www.w3.org/2004/02/skos/core#prefLabel> "Time Resolved Ultra-Small Angle X-ray Scattering" .


###  http://purl.org/pan-science/ESRFET#TR-XRD
:TR-XRD rdf:type owl:Class ;
        rdfs:subClassOf :experimental_technique ;
        rdfs:comment "Time-Resolved X-ray Diffraction (TR-XRD) measures changes in X-ray diffraction patterns as a function of time to study dynamic processes such as phase transitions, chemical reactions, and structural changes in materials." ;
        rdfs:label "TR-XRD" ;
        <http://www.w3.org/2004/02/skos/core#prefLabel> "Time Resolved X-ray Diffraction" .


###  http://purl.org/pan-science/ESRFET#TR-XSS
:TR-XSS rdf:type owl:Class ;
        owl:equivalentClass [ owl:intersectionOf ( :experimental_technique
                                                   [ rdf:type owl:Restriction ;
                                                     owl:onProperty :measures_as_a_function_of ;
                                                     owl:someValuesFrom :detection_as_a_function_of_time
                                                   ]
                                                   [ rdf:type owl:Restriction ;
                                                     owl:onProperty :measures_result_of_interaction ;
                                                     owl:someValuesFrom :diffraction_of_elastic_scattering
                                                   ]
                                                   [ rdf:type owl:Restriction ;
                                                     owl:onProperty :requires_sample_input ;
                                                     owl:someValuesFrom :x-ray
                                                   ]
                                                   [ rdf:type owl:Restriction ;
                                                     owl:onProperty :requires_sample_type ;
                                                     owl:someValuesFrom :chemical_solution
                                                   ]
                                                 ) ;
                              rdf:type owl:Class
                            ] ;
        rdfs:comment "Time-Resolved X-ray Solution Scattering (TR-XSS) measures transient changes in X-ray scattering from a solution of chemicals or biomolecules following a triggering perturbation, providing insights into the dynamics of structural rearrangements of the solute and of the surrounding solvent." ;
        rdfs:label "TR-XSS" ;
        <http://www.w3.org/2004/02/skos/core#prefLabel> "Time-resolved X-ray solution scattering" .


###  http://purl.org/pan-science/ESRFET#TXRF
:TXRF rdf:type owl:Class ;
      owl:equivalentClass [ owl:intersectionOf ( :experimental_technique
                                                 [ rdf:type owl:Restriction ;
                                                   owl:onProperty :measures_interaction_result_property ;
                                                   owl:someValuesFrom :photon_count
                                                 ]
                                                 [ rdf:type owl:Restriction ;
                                                   owl:onProperty :measures_interaction_result_property ;
                                                   owl:someValuesFrom :photon_energy
                                                 ]
                                                 [ rdf:type owl:Restriction ;
                                                   owl:onProperty :measures_result_of_interaction ;
                                                   owl:someValuesFrom :fluorescence
                                                 ]
                                                 [ rdf:type owl:Restriction ;
                                                   owl:onProperty :requires_sample_input ;
                                                   owl:someValuesFrom :x-ray
                                                 ]
                                                 [ rdf:type owl:Restriction ;
                                                   owl:onProperty :requires_sample_input_property ;
                                                   owl:someValuesFrom :sample_incident_angle_smaller_than_critical_angle
                                                 ]
                                               ) ;
                            rdf:type owl:Class
                          ] ;
      rdfs:comment "Total Reflection X-ray Fluorescence (TXRF) measures characteristic X-rays emitted by a sample under total external reflection conditions, providing highly sensitive, surface-specific elemental analysis with minimal sample preparation." ;
      rdfs:label "TXRF" ;
      <http://www.w3.org/2004/02/skos/core#prefLabel> "Total Reflection X-ray Fluorescence" .


###  http://purl.org/pan-science/ESRFET#USA-XPCS
:USA-XPCS rdf:type owl:Class ;
          rdfs:subClassOf :experimental_technique ;
          rdfs:comment "Ultra-Small Angle X-ray Photon Correlation Spectroscopy (USA-XPCS) measures time-dependent fluctuations of coherent X-ray scattering at ultra-small angles to probe slow dynamics and structural rearrangements on large length scales in complex materials." ;
          rdfs:label "USA-XPCS" ;
          <http://www.w3.org/2004/02/skos/core#prefLabel> "Ultra-Small Angle X-ray Photon Correlation Spectroscopy" .


###  http://purl.org/pan-science/ESRFET#USAXS
:USAXS rdf:type owl:Class ;
       owl:equivalentClass [ owl:intersectionOf ( :experimental_technique
                                                  [ rdf:type owl:Restriction ;
                                                    owl:onProperty :measures_interaction_result_property ;
                                                    owl:someValuesFrom :ultra_large_length_scales
                                                  ]
                                                  [ rdf:type owl:Restriction ;
                                                    owl:onProperty :measures_result_of_interaction ;
                                                    owl:someValuesFrom :diffraction_of_elastic_scattering
                                                  ]
                                                  [ rdf:type owl:Restriction ;
                                                    owl:onProperty :requires_sample_input ;
                                                    owl:someValuesFrom :x-ray
                                                  ]
                                                ) ;
                             rdf:type owl:Class
                           ] ;
       rdfs:comment "Ultra-Small Angle X-ray Scattering (USAXS) measures X-ray scattering at extremely small angles to probe structural features on length scales larger than those accessible by SAXS, such as large-scale aggregates, pores, or hierarchical structures." ;
       rdfs:label "USAXS" ;
       <http://www.w3.org/2004/02/skos/core#prefLabel> "Ultra-Small Angle X-ray Scattering" .


###  http://purl.org/pan-science/ESRFET#UV
:UV rdf:type owl:Class ;
    rdfs:subClassOf :named_photon_energy_ranges .


###  http://purl.org/pan-science/ESRFET#VLM
:VLM rdf:type owl:Class ;
     owl:equivalentClass [ owl:intersectionOf ( :experimental_technique
                                                [ rdf:type owl:Restriction ;
                                                  owl:onProperty :measures_as_a_function_of ;
                                                  owl:someValuesFrom :full-field_imaging
                                                ]
                                                [ rdf:type owl:Restriction ;
                                                  owl:onProperty :measures_as_a_function_of ;
                                                  owl:someValuesFrom :micro_sample_spatial_resolution
                                                ]
                                                [ rdf:type owl:Restriction ;
                                                  owl:onProperty :requires_sample_input ;
                                                  owl:someValuesFrom :visual_spectrum
                                                ]
                                              ) ;
                           rdf:type owl:Class
                         ] ;
     rdfs:comment "Visible Light Microscopy (VLM) captures images of a sample using visible light illumination and optical lenses, providing spatially resolved information about surface morphology, color, and structure at micrometer-scale resolution." ;
     rdfs:label "VLM" ;
     <http://www.w3.org/2004/02/skos/core#prefLabel> "Visible Light Microscopy" .


###  http://purl.org/pan-science/ESRFET#WAXS
:WAXS rdf:type owl:Class ;
      owl:equivalentClass [ owl:intersectionOf ( :experimental_technique
                                                 [ rdf:type owl:Restriction ;
                                                   owl:onProperty :measures_interaction_result_property ;
                                                   owl:someValuesFrom :small_length_scales
                                                 ]
                                                 [ rdf:type owl:Restriction ;
                                                   owl:onProperty :measures_result_of_interaction ;
                                                   owl:someValuesFrom :diffraction_of_elastic_scattering
                                                 ]
                                                 [ rdf:type owl:Restriction ;
                                                   owl:onProperty :requires_sample_input ;
                                                   owl:someValuesFrom :x-ray
                                                 ]
                                               ) ;
                            rdf:type owl:Class
                          ] ;
      rdfs:comment "Wide-Angle X-ray Scattering (WAXS) measures X-ray scattering at larger angles than SAXS to provide information on short-range order, crystalline structure, and molecular packing in materials." ;
      rdfs:label "WAXS" ;
      <http://www.w3.org/2004/02/skos/core#prefLabel> "Wide-angle X-ray Scattering" .


###  http://purl.org/pan-science/ESRFET#WDS
:WDS rdf:type owl:Class ;
     owl:equivalentClass [ owl:intersectionOf ( :experimental_technique
                                                [ rdf:type owl:Restriction ;
                                                  owl:onProperty :measures_interaction_result_property ;
                                                  owl:someValuesFrom :photon_count
                                                ]
                                                [ rdf:type owl:Restriction ;
                                                  owl:onProperty :measures_interaction_result_property ;
                                                  owl:someValuesFrom :photon_energy
                                                ]
                                                [ rdf:type owl:Restriction ;
                                                  owl:onProperty :measures_result_of_interaction ;
                                                  owl:someValuesFrom :fluorescence
                                                ]
                                                [ rdf:type owl:Restriction ;
                                                  owl:onProperty :measures_with_a_detector_type ;
                                                  owl:someValuesFrom :wavelength_dispersive_detector
                                                ]
                                                [ rdf:type owl:Restriction ;
                                                  owl:onProperty :requires_sample_input ;
                                                  owl:someValuesFrom :x-ray
                                                ]
                                              ) ;
                           rdf:type owl:Class
                         ] ;
     rdfs:comment "WDS measures X-ray photons coming from a sample during irradition with a wavelength dispersive detector and derives elemental composition from the energy of the fluorescence photons" ;
     rdfs:label "WDS" ;
     <http://www.w3.org/2004/02/skos/core#prefLabel> "Wavelength Dispersive X-ray Spectroscopy" .


###  http://purl.org/pan-science/ESRFET#XACT
:XACT rdf:type owl:Class ;
      owl:equivalentClass [ owl:intersectionOf ( :experimental_technique
                                                 [ rdf:type owl:Restriction ;
                                                   owl:onProperty :measures_as_a_function_of ;
                                                   owl:someValuesFrom :tomography
                                                 ]
                                                 [ rdf:type owl:Restriction ;
                                                   owl:onProperty :measures_result_of_interaction ;
                                                   owl:someValuesFrom :transmission
                                                 ]
                                                 [ rdf:type owl:Restriction ;
                                                   owl:onProperty :requires_sample_input ;
                                                   owl:someValuesFrom :x-ray
                                                 ]
                                               ) ;
                            rdf:type owl:Class
                          ] ;
      rdfs:comment "X-ray Absorption Tomography measures X-ray attenuation through a sample from multiple projection angles and reconstructs a 3D map of the absorption coefficient, revealing internal density variations within the material." ;
      rdfs:label "XACT" ;
      <http://www.w3.org/2004/02/skos/core#prefLabel> "X-ray Absorption Tomography" .


###  http://purl.org/pan-science/ESRFET#XANES
:XANES rdf:type owl:Class ;
       owl:equivalentClass [ owl:intersectionOf ( :experimental_technique
                                                  [ rdf:type owl:Restriction ;
                                                    owl:onProperty :measures_as_a_function_of ;
                                                    owl:someValuesFrom :near_edge
                                                  ]
                                                  [ rdf:type owl:Restriction ;
                                                    owl:onProperty :measures_interaction_result_property ;
                                                    owl:someValuesFrom :photon_count
                                                  ]
                                                  [ rdf:type owl:Restriction ;
                                                    owl:onProperty :measures_result_of_interaction ;
                                                    owl:someValuesFrom :atomic_core_excitation
                                                  ]
                                                  [ rdf:type owl:Restriction ;
                                                    owl:onProperty :requires_sample_input ;
                                                    owl:someValuesFrom :x-ray
                                                  ]
                                                ) ;
                             rdf:type owl:Class
                           ] ;
       rdfs:comment "XANES (X-ray Absorption Near Edge Structure) measures the fine structure in X-ray absorption near an element’s absorption edge, providing information about the oxidation state, electronic structure, and coordination geometry of the absorbing atoms." ;
       rdfs:label "XANES" ;
       <http://www.w3.org/2004/02/skos/core#prefLabel> "X-ray Absorption Near Edge Structure" .


###  http://purl.org/pan-science/ESRFET#XAPCT
:XAPCT rdf:type owl:Class ;
       owl:equivalentClass [ owl:intersectionOf ( :experimental_technique
                                                  [ rdf:type owl:Restriction ;
                                                    owl:onProperty :measures_as_a_function_of ;
                                                    owl:someValuesFrom :tomography
                                                  ]
                                                  [ rdf:type owl:Restriction ;
                                                    owl:onProperty :measures_result_of_interaction ;
                                                    owl:someValuesFrom :diffraction_of_elastic_scattering
                                                  ]
                                                  [ rdf:type owl:Restriction ;
                                                    owl:onProperty :measures_result_of_interaction ;
                                                    owl:someValuesFrom :diffusion
                                                  ]
                                                  [ rdf:type owl:Restriction ;
                                                    owl:onProperty :measures_result_of_interaction ;
                                                    owl:someValuesFrom :refraction
                                                  ]
                                                  [ rdf:type owl:Restriction ;
                                                    owl:onProperty :measures_result_of_interaction ;
                                                    owl:someValuesFrom :transmission
                                                  ]
                                                  [ rdf:type owl:Restriction ;
                                                    owl:onProperty :measures_with_a_detector_type ;
                                                    owl:someValuesFrom :analyzer_crystal
                                                  ]
                                                  [ rdf:type owl:Restriction ;
                                                    owl:onProperty :requires_sample_input ;
                                                    owl:someValuesFrom :monochromatic_beam
                                                  ]
                                                  [ rdf:type owl:Restriction ;
                                                    owl:onProperty :requires_sample_input ;
                                                    owl:someValuesFrom :x-ray
                                                  ]
                                                ) ;
                             rdf:type owl:Class
                           ] ;
       rdfs:comment "X-ray Analyzer-Based Phase-Contrast Tomography (XAPCT) measures angular deviations of X-rays transmitted through a sample using a crystal analyzer to map phase gradients, providing 3D images with high contrast for interfaces and internal structures." ;
       rdfs:label "XAPCT" ;
       <http://www.w3.org/2004/02/skos/core#prefLabel> "X-ray Analyzer-Based Phase-Contrast Tomography" .


###  http://purl.org/pan-science/ESRFET#XAS
:XAS rdf:type owl:Class ;
     owl:equivalentClass [ owl:intersectionOf ( :experimental_technique
                                                [ rdf:type owl:Restriction ;
                                                  owl:onProperty :measures_as_a_function_of ;
                                                  owl:someValuesFrom :detection_as_a_function_of_incident_energy
                                                ]
                                                [ rdf:type owl:Restriction ;
                                                  owl:onProperty :measures_interaction_result_property ;
                                                  owl:someValuesFrom :photon_count
                                                ]
                                                [ rdf:type owl:Restriction ;
                                                  owl:onProperty :measures_result_of_interaction ;
                                                  owl:someValuesFrom :atomic_core_excitation
                                                ]
                                                [ rdf:type owl:Restriction ;
                                                  owl:onProperty :requires_sample_input ;
                                                  owl:someValuesFrom :x-ray
                                                ]
                                              ) ;
                           rdf:type owl:Class
                         ] ;
     rdfs:comment "XAS measures a signal related to the X-ray absorption probability—such as fluorescence, photon electrons, Auger electrons, or transmission—as a function of the incident X-ray photon energy. It probes atomic core-level excitations by removing core-shell electrons, providing element-specific information about the local chemical environment, oxidation state, and atomic structure around the absorbing atoms." ;
     rdfs:label "XAS" ;
     <http://www.w3.org/2004/02/skos/core#prefLabel> "X-ray Absorption Spectroscopy" .


###  http://purl.org/pan-science/ESRFET#XBH
:XBH rdf:type owl:Class ;
     rdfs:subClassOf :experimental_technique ;
     rdfs:comment "X-ray Bragg Holography (XBH) measures interference patterns formed by Bragg-diffracted and reference X-rays from a crystal to reconstruct 3D atomic-scale images of the crystal structure." ;
     rdfs:label "XBH" ;
     <http://www.w3.org/2004/02/skos/core#prefLabel> "X-ray Bragg Holography" .


###  http://purl.org/pan-science/ESRFET#XCL
:XCL rdf:type owl:Class ;
     owl:equivalentClass [ owl:intersectionOf ( :experimental_technique
                                                [ rdf:type owl:Restriction ;
                                                  owl:onProperty :measures_as_a_function_of ;
                                                  owl:someValuesFrom :laminography
                                                ]
                                                [ rdf:type owl:Restriction ;
                                                  owl:onProperty :requires_sample_input ;
                                                  owl:someValuesFrom :x-ray
                                                ]
                                              ) ;
                           rdf:type owl:Class
                         ] ;
     rdfs:comment "X-ray Computed Laminography (XCL) measures the interaction of X-rays with flat or extended samples (through absorption, phase, or scattering contrast) at multiple tilted angles to reconstruct 3D images of internal structures that are difficult to access with conventional tomography due to sample geometry." ;
     rdfs:label "XCL" ;
     <http://www.w3.org/2004/02/skos/core#prefLabel> "X-ray Computed Laminography" .


###  http://purl.org/pan-science/ESRFET#XDMR
:XDMR rdf:type owl:Class ;
      rdfs:subClassOf :experimental_technique ;
      rdfs:comment "X-ray Detected Magnetic Resonance (XDMR) measures changes in X-ray absorption or emission induced by magnetic resonance excitation, providing element-specific information on spin dynamics and magnetic excitations." ;
      rdfs:label "XDMR" ;
      <http://www.w3.org/2004/02/skos/core#prefLabel> "X-ray Detected Magnetic Resonance" .


###  http://purl.org/pan-science/ESRFET#XDS
:XDS rdf:type owl:Class ;
     rdfs:subClassOf :experimental_technique ;
     rdfs:comment "X-ray Diffuse Scattering (XDS) measures scattered X-rays away from Bragg peaks to probe local disorder, defects, thermal vibrations, and nanoscale structural fluctuations in materials." ;
     rdfs:label "XDS" ;
     <http://www.w3.org/2004/02/skos/core#prefLabel> "X-ray Diffuse Scattering" .


###  http://purl.org/pan-science/ESRFET#XEOL
:XEOL rdf:type owl:Class ;
      rdfs:subClassOf :experimental_technique ;
      rdfs:comment "X-ray Excited Optical Luminescence (XEOL) measures visible or near-visible light emitted from a sample after X-ray excitation, providing information on electronic structure, defect states, and luminescent centers." ;
      rdfs:label "XEOL" ;
      <http://www.w3.org/2004/02/skos/core#prefLabel> "X-ray Excited Optical Luminescence" .


###  http://purl.org/pan-science/ESRFET#XES
:XES rdf:type owl:Class ;
     rdfs:subClassOf :experimental_technique ;
     rdfs:comment "X-ray Emission Spectroscopy (XES) measures emitted X-ray photons from electronic transitions after X-ray excitation, revealing detailed information about the electronic structure and chemical state of elements. Unlike XRF, which identifies elemental composition through broad characteristic fluorescence lines, XES uses high energy resolution to resolve fine spectral features—such as valence-to-core transitions—providing deeper insight into the local chemical bonding and electronic environment." ;
     rdfs:label "XES" ;
     <http://www.w3.org/2004/02/skos/core#prefLabel> "X-ray Emission Spectroscopy" .


###  http://purl.org/pan-science/ESRFET#XFCT
:XFCT rdf:type owl:Class ;
      owl:equivalentClass [ owl:intersectionOf ( :experimental_technique
                                                 [ rdf:type owl:Restriction ;
                                                   owl:onProperty :measures_as_a_function_of ;
                                                   owl:someValuesFrom :tomography
                                                 ]
                                                 [ rdf:type owl:Restriction ;
                                                   owl:onProperty :measures_interaction_result_property ;
                                                   owl:someValuesFrom :photon_count
                                                 ]
                                                 [ rdf:type owl:Restriction ;
                                                   owl:onProperty :measures_interaction_result_property ;
                                                   owl:someValuesFrom :photon_energy
                                                 ]
                                                 [ rdf:type owl:Restriction ;
                                                   owl:onProperty :measures_result_of_interaction ;
                                                   owl:someValuesFrom :fluorescence
                                                 ]
                                                 [ rdf:type owl:Restriction ;
                                                   owl:onProperty :requires_sample_input ;
                                                   owl:someValuesFrom :x-ray
                                                 ]
                                               ) ;
                            rdf:type owl:Class
                          ] ;
      rdfs:comment "X-ray Fluorescence Tomography (XFCT) measures characteristic fluorescence X-rays emitted from a sample at multiple angles to reconstruct 3D elemental distributions with high sensitivity and spatial resolution." ;
      rdfs:label "XFCT" ;
      <http://www.w3.org/2004/02/skos/core#prefLabel> "X-ray Fluorescence Tomography" .


###  http://purl.org/pan-science/ESRFET#XFH
:XFH rdf:type owl:Class ;
     rdfs:subClassOf :experimental_technique ;
     rdfs:comment "X-ray Fluorescence Holography (XFH) measures interference between fluorescent X-rays emitted from atoms and scattered reference waves to obtain 3D atomic-scale images of the local atomic arrangement around specific elements." ;
     rdfs:label "XFH" ;
     <http://www.w3.org/2004/02/skos/core#prefLabel> "X-ray Fluorescence Holography" .


###  http://purl.org/pan-science/ESRFET#XGI
:XGI rdf:type owl:Class ;
     owl:equivalentClass [ owl:intersectionOf ( :experimental_technique
                                                [ rdf:type owl:Restriction ;
                                                  owl:onProperty :measures_as_a_function_of ;
                                                  owl:someValuesFrom :simultanious_reference
                                                ]
                                                [ rdf:type owl:Restriction ;
                                                  owl:onProperty :measures_as_a_function_of ;
                                                  owl:someValuesFrom <http://purl.org/pan-science/PaNET/PaNET01106>
                                                ]
                                                [ rdf:type owl:Restriction ;
                                                  owl:onProperty :measures_result_of_interaction ;
                                                  owl:someValuesFrom :diffusion
                                                ]
                                                [ rdf:type owl:Restriction ;
                                                  owl:onProperty :measures_result_of_interaction ;
                                                  owl:someValuesFrom :refraction
                                                ]
                                                [ rdf:type owl:Restriction ;
                                                  owl:onProperty :measures_result_of_interaction ;
                                                  owl:someValuesFrom :transmission
                                                ]
                                                [ rdf:type owl:Restriction ;
                                                  owl:onProperty :requires_sample_input ;
                                                  owl:someValuesFrom :x-ray
                                                ]
                                                [ rdf:type owl:Restriction ;
                                                  owl:onProperty :requires_sample_input_property ;
                                                  owl:someValuesFrom :speckle_pattern
                                                ]
                                              ) ;
                           rdf:type owl:Class
                         ] ;
     rdfs:subClassOf :experimental_technique ;
     rdfs:comment "X-ray Ghost Imaging (XGI) measures correlations between structured illumination patterns and total transmitted intensities to reconstruct 2D or 3D images without spatially resolved detection. Unlike speckle imaging, ghost imaging simultaneously records reference (without sample) and sample-affected signals using a beam splitter." ;
     rdfs:label "XGI" ;
     <http://www.w3.org/2004/02/skos/core#prefLabel> "X-ray Ghost Imaging" .


###  http://purl.org/pan-science/ESRFET#XGPCT
:XGPCT rdf:type owl:Class ;
       owl:equivalentClass [ owl:intersectionOf ( :experimental_technique
                                                  [ rdf:type owl:Restriction ;
                                                    owl:onProperty :measures_as_a_function_of ;
                                                    owl:someValuesFrom :tomography
                                                  ]
                                                  [ rdf:type owl:Restriction ;
                                                    owl:onProperty :measures_result_of_interaction ;
                                                    owl:someValuesFrom :diffusion
                                                  ]
                                                  [ rdf:type owl:Restriction ;
                                                    owl:onProperty :measures_result_of_interaction ;
                                                    owl:someValuesFrom :refraction
                                                  ]
                                                  [ rdf:type owl:Restriction ;
                                                    owl:onProperty :measures_result_of_interaction ;
                                                    owl:someValuesFrom :transmission
                                                  ]
                                                  [ rdf:type owl:Restriction ;
                                                    owl:onProperty :requires_sample_input ;
                                                    owl:someValuesFrom :x-ray
                                                  ]
                                                  [ rdf:type owl:Restriction ;
                                                    owl:onProperty :requires_sample_input_property ;
                                                    owl:someValuesFrom :grating
                                                  ]
                                                ) ;
                             rdf:type owl:Class
                           ] ;
       rdfs:comment "X-ray Grating Phase-Contrast Tomography (XGPCT) measures X-ray phase shifts using an interferometric grating setup across multiple projection angles, providing 3D images with high sensitivity to small refractive index variations in soft or low-Z materials." ;
       rdfs:label "XGPCT" ;
       <http://www.w3.org/2004/02/skos/core#prefLabel> "X-ray Grating Phase-Contrast Tomography" .


###  http://purl.org/pan-science/ESRFET#XHT
:XHT rdf:type owl:Class ;
     owl:equivalentClass [ owl:intersectionOf ( :experimental_technique
                                                [ rdf:type owl:Restriction ;
                                                  owl:onProperty :measures_as_a_function_of ;
                                                  owl:someValuesFrom :detection_as_a_function_of_limited_number_of_sample_to_detector_distance
                                                ]
                                                [ rdf:type owl:Restriction ;
                                                  owl:onProperty :measures_as_a_function_of ;
                                                  owl:someValuesFrom :tomography
                                                ]
                                                [ rdf:type owl:Restriction ;
                                                  owl:onProperty :measures_result_of_interaction ;
                                                  owl:someValuesFrom :refraction
                                                ]
                                                [ rdf:type owl:Restriction ;
                                                  owl:onProperty :measures_result_of_interaction ;
                                                  owl:someValuesFrom :transmission
                                                ]
                                                [ rdf:type owl:Restriction ;
                                                  owl:onProperty :requires_sample_input ;
                                                  owl:someValuesFrom :x-ray
                                                ]
                                                [ rdf:type owl:Restriction ;
                                                  owl:onProperty :requires_sample_input_property ;
                                                  owl:someValuesFrom :unmodified_beam
                                                ]
                                              ) ;
                           rdf:type owl:Class
                         ] ;
     rdfs:comment "X-ray HoloTomography (XHT) combines holographic imaging and tomography by recording holograms at multiple sample–detector distances and projection angles to reconstruct 3D electron density maps with sub-micrometer resolution." ;
     rdfs:label "XHT" ;
     <http://www.w3.org/2004/02/skos/core#prefLabel> "X-ray HoloTomography" .


###  http://purl.org/pan-science/ESRFET#XLD
:XLD rdf:type owl:Class ;
     rdfs:subClassOf :experimental_technique ;
     rdfs:comment "X-ray Linear Dichroism (XLD) measures the difference in X-ray absorption for linearly polarized light oriented along different crystallographic axes, providing information on electronic anisotropy and orbital ordering." ;
     rdfs:label "XLD" ;
     <http://www.w3.org/2004/02/skos/core#prefLabel> "X-ray Linear Dichroism" .


###  http://purl.org/pan-science/ESRFET#XMCD
:XMCD rdf:type owl:Class ;
      rdfs:subClassOf :experimental_technique ;
      rdfs:comment "X-ray Magnetic Circular Dichroism (XMCD) measures the difference in absorption of left- and right-circularly polarized X-rays in a magnetized sample, probing element-specific magnetic moments and spin states." ;
      rdfs:label "XMCD" ;
      <http://www.w3.org/2004/02/skos/core#prefLabel> "X-ray Magnetic Circular Dichroism" .


###  http://purl.org/pan-science/ESRFET#XMLD
:XMLD rdf:type owl:Class ;
      rdfs:subClassOf :experimental_technique ;
      rdfs:comment "X-ray Magnetic Linear Dichroism (XMLD) measures differences in X-ray absorption of linearly polarized light depending on magnetic order, sensitive to antiferromagnetic and magnetic domain structures." ;
      rdfs:label "XMLD" ;
      <http://www.w3.org/2004/02/skos/core#prefLabel> "X-ray Magnetic Linear Dichroism" .


###  http://purl.org/pan-science/ESRFET#XMχD
:XMχD rdf:type owl:Class ;
      rdfs:subClassOf :experimental_technique ;
      rdfs:comment "X-ray MagnetoChiral Dichroism (XMχD) measures differences in X-ray absorption related to the combined effects of magnetism and chirality in materials, revealing chiral magnetic structures." ;
      rdfs:label "XMχD" ;
      <http://www.w3.org/2004/02/skos/core#prefLabel> "X-ray MagnetoChiral Dichroism" .


###  http://purl.org/pan-science/ESRFET#XNCD
:XNCD rdf:type owl:Class ;
      rdfs:subClassOf :experimental_technique ;
      rdfs:comment "X-ray Natural Circular Dichroism (XNCD) measures differences in absorption of circularly polarized X-rays in non-magnetic chiral materials, providing information on structural chirality and electronic asymmetry." ;
      rdfs:label "XNCD" ;
      <http://www.w3.org/2004/02/skos/core#prefLabel> "X-ray Natural Circular Dichroism" .


###  http://purl.org/pan-science/ESRFET#XNHT
:XNHT rdf:type owl:Class ;
      owl:equivalentClass [ owl:intersectionOf ( :experimental_technique
                                                 [ rdf:type owl:Restriction ;
                                                   owl:onProperty :measures_as_a_function_of ;
                                                   owl:someValuesFrom :detection_as_a_function_of_limited_number_of_sample_to_detector_distance
                                                 ]
                                                 [ rdf:type owl:Restriction ;
                                                   owl:onProperty :measures_as_a_function_of ;
                                                   owl:someValuesFrom :nano_sample_spatial_resolution
                                                 ]
                                                 [ rdf:type owl:Restriction ;
                                                   owl:onProperty :measures_as_a_function_of ;
                                                   owl:someValuesFrom :tomography
                                                 ]
                                                 [ rdf:type owl:Restriction ;
                                                   owl:onProperty :measures_result_of_interaction ;
                                                   owl:someValuesFrom :refraction
                                                 ]
                                                 [ rdf:type owl:Restriction ;
                                                   owl:onProperty :measures_result_of_interaction ;
                                                   owl:someValuesFrom :transmission
                                                 ]
                                                 [ rdf:type owl:Restriction ;
                                                   owl:onProperty :requires_sample_input ;
                                                   owl:someValuesFrom :x-ray
                                                 ]
                                                 [ rdf:type owl:Restriction ;
                                                   owl:onProperty :requires_sample_input_property ;
                                                   owl:someValuesFrom :unmodified_beam
                                                 ]
                                               ) ;
                            rdf:type owl:Class
                          ] ;
      rdfs:comment "X-ray Nano-HoloTomography (XNHT) is a high-resolution variant of XHT that combines nanoscale focusing and holographic tomography to obtain 3D electron density maps of internal structure at nanometer resolution." ;
      rdfs:label "XNHT" ;
      <http://www.w3.org/2004/02/skos/core#prefLabel> "X-ray Nano-HoloTomography" .


###  http://purl.org/pan-science/ESRFET#XPCI
:XPCI rdf:type owl:Class ;
      rdfs:subClassOf :experimental_technique ;
      rdfs:comment "X-ray Phase-Contrast Imaging (XPCI) measures phase shifts of X-rays transmitted through a sample to enhance image contrast, enabling visualization of structures with low absorption contrast such as soft tissues or light materials." ;
      rdfs:label "XPCI" ;
      <http://www.w3.org/2004/02/skos/core#altLabel> "PCXI" ,
                                                     "Phase-Contrast X-ray Imaging" ;
      <http://www.w3.org/2004/02/skos/core#prefLabel> "X-ray Phase-Contrast Imaging" .


###  http://purl.org/pan-science/ESRFET#XPCS
:XPCS rdf:type owl:Class ;
      rdfs:subClassOf :experimental_technique ;
      rdfs:comment "X-ray Photon Correlation Spectroscopy (XPCS) measures time fluctuations of coherent X-ray scattering intensity to probe nanoscale dynamics and temporal correlations in materials such as particle motion, phase transitions, or relaxation processes." ;
      rdfs:label "XPCS" ;
      <http://www.w3.org/2004/02/skos/core#prefLabel> "X-ray Photon Correlation Spectroscopy" .


###  http://purl.org/pan-science/ESRFET#XPCT
:XPCT rdf:type owl:Class ;
      owl:equivalentClass [ owl:intersectionOf ( :experimental_technique
                                                 [ rdf:type owl:Restriction ;
                                                   owl:onProperty :measures_as_a_function_of ;
                                                   owl:someValuesFrom :tomography
                                                 ]
                                                 [ rdf:type owl:Restriction ;
                                                   owl:onProperty :measures_result_of_interaction ;
                                                   owl:someValuesFrom :refraction
                                                 ]
                                                 [ rdf:type owl:Restriction ;
                                                   owl:onProperty :measures_result_of_interaction ;
                                                   owl:someValuesFrom :transmission
                                                 ]
                                                 [ rdf:type owl:Restriction ;
                                                   owl:onProperty :requires_sample_input ;
                                                   owl:someValuesFrom :x-ray
                                                 ]
                                               ) ;
                            rdf:type owl:Class
                          ] ;
      rdfs:comment "X-ray Phase-Contrast Tomography (XPCT) measures phase shifts of X-rays passing through a sample from multiple angles to reconstruct 3D images with enhanced contrast for weakly absorbing materials, revealing internal structures invisible in conventional absorption tomography." ;
      rdfs:label "XPCT" ;
      <http://www.w3.org/2004/02/skos/core#prefLabel> "Phase-Contrast Tomography" .


###  http://purl.org/pan-science/ESRFET#XPS
:XPS rdf:type owl:Class ;
     rdfs:subClassOf :experimental_technique ;
     rdfs:comment "X-ray Photoelectron Spectroscopy (XPS) measures the kinetic energy of electrons ejected by X-rays to determine elemental composition and chemical states near the surface of a material." ;
     rdfs:label "XPS" ;
     <http://www.w3.org/2004/02/skos/core#prefLabel> "X-ray Photoelectron Spectroscopy" .


###  http://purl.org/pan-science/ESRFET#XRAYS
:XRAYS rdf:type owl:Class ;
       owl:equivalentClass [ owl:intersectionOf ( :experimental_technique
                                                  [ rdf:type owl:Restriction ;
                                                    owl:onProperty :requires_sample_input ;
                                                    owl:someValuesFrom :x-ray
                                                  ]
                                                ) ;
                             rdf:type owl:Class
                           ] ;
       rdfs:subClassOf :experimental_technique ;
       rdfs:comment "Experimental techniques based on irradiating a sample with X-rays to probe its properties by measuring interactions such as absorption, scattering, fluorescence, or diffraction, providing insights into structural, elemental, or electronic characteristics depending on the specific method used." ;
       rdfs:label "XRAYS" ;
       <http://www.w3.org/2004/02/skos/core#prefLabel> "X-ray Radiation Technique" .


###  http://purl.org/pan-science/ESRFET#XRCT
:XRCT rdf:type owl:Class ;
      owl:equivalentClass [ owl:intersectionOf ( :experimental_technique
                                                 [ rdf:type owl:Restriction ;
                                                   owl:onProperty :measures_as_a_function_of ;
                                                   owl:someValuesFrom :tomography
                                                 ]
                                                 [ rdf:type owl:Restriction ;
                                                   owl:onProperty :requires_sample_input ;
                                                   owl:someValuesFrom :x-ray
                                                 ]
                                               ) ;
                            rdf:type owl:Class
                          ] ;
      rdfs:comment "X-ray Computed Tomography (XRCT) measures the interaction of X-rays with a sample (through absorption, phase, or scattering contrast) from multiple angles to reconstruct a 3D volume, providing detailed internal structural information such as density, morphology, and defects." ;
      rdfs:label "XRCT" ;
      <http://www.w3.org/2004/02/skos/core#prefLabel> "X-ray Computed Tomography" .


###  http://purl.org/pan-science/ESRFET#XRD
:XRD rdf:type owl:Class ;
     owl:equivalentClass [ owl:intersectionOf ( :experimental_technique
                                                [ rdf:type owl:Restriction ;
                                                  owl:onProperty :measures_result_of_interaction ;
                                                  owl:someValuesFrom :diffraction_of_elastic_scattering
                                                ]
                                                [ rdf:type owl:Restriction ;
                                                  owl:onProperty :requires_sample_input ;
                                                  owl:someValuesFrom :x-ray
                                                ]
                                              ) ;
                           rdf:type owl:Class
                         ] ;
     rdfs:comment "X-ray Diffraction (XRD) measures the diffraction pattern produced when X-rays interact with a crystalline sample. The pattern provides information about the crystal structure, phase identification, lattice parameters, and crystallite size of the material." ;
     rdfs:label "XRD" ;
     <http://www.w3.org/2004/02/skos/core#prefLabel> "X-ray diffraction" .


###  http://purl.org/pan-science/ESRFET#XRF
:XRF rdf:type owl:Class ;
     owl:equivalentClass [ owl:intersectionOf ( :experimental_technique
                                                [ rdf:type owl:Restriction ;
                                                  owl:onProperty :measures_interaction_result_property ;
                                                  owl:someValuesFrom :photon_count
                                                ]
                                                [ rdf:type owl:Restriction ;
                                                  owl:onProperty :measures_interaction_result_property ;
                                                  owl:someValuesFrom :photon_energy
                                                ]
                                                [ rdf:type owl:Restriction ;
                                                  owl:onProperty :measures_result_of_interaction ;
                                                  owl:someValuesFrom :fluorescence
                                                ]
                                                [ rdf:type owl:Restriction ;
                                                  owl:onProperty :requires_sample_input ;
                                                  owl:someValuesFrom :x-ray
                                                ]
                                              ) ;
                           rdf:type owl:Class
                         ] ;
     rdfs:comment "X-ray Fluorescence (XRF) measures characteristic X-ray photons emitted by a sample when it is irradiated with X-rays. The energy of the emitted fluorescence photons reveals the elemental composition and chemical state of the sample." ;
     rdfs:label "XRF" ;
     <http://www.w3.org/2004/02/skos/core#prefLabel> "X-ray Fluorescence Spectroscopy" .


###  http://purl.org/pan-science/ESRFET#XRPD
:XRPD rdf:type owl:Class ;
      owl:equivalentClass [ owl:intersectionOf ( :experimental_technique
                                                 [ rdf:type owl:Restriction ;
                                                   owl:onProperty :measures_result_of_interaction ;
                                                   owl:someValuesFrom :diffraction_of_elastic_scattering
                                                 ]
                                                 [ rdf:type owl:Restriction ;
                                                   owl:onProperty :requires_sample_input ;
                                                   owl:someValuesFrom :x-ray
                                                 ]
                                                 [ rdf:type owl:Restriction ;
                                                   owl:onProperty :requires_sample_type ;
                                                   owl:someValuesFrom :powder_sample
                                                 ]
                                               ) ;
                            rdf:type owl:Class
                          ] ;
      rdfs:subClassOf :experimental_technique ;
      rdfs:comment "X-ray Powder Diffraction (XRPD) measures diffraction patterns from polycrystalline or powdered samples to identify phases, determine crystal structure, lattice parameters, and quantify phase composition." ;
      rdfs:label "XRPD" ;
      <http://www.w3.org/2004/02/skos/core#prefLabel> "X-ray Powder Diffraction" .


###  http://purl.org/pan-science/ESRFET#XRR
:XRR rdf:type owl:Class ;
     owl:equivalentClass [ owl:intersectionOf ( :experimental_technique
                                                [ rdf:type owl:Restriction ;
                                                  owl:onProperty :measures_result_of_interaction ;
                                                  owl:someValuesFrom :reflection
                                                ]
                                                [ rdf:type owl:Restriction ;
                                                  owl:onProperty :requires_sample_input ;
                                                  owl:someValuesFrom :x-ray
                                                ]
                                              ) ;
                           rdf:type owl:Class
                         ] ;
     rdfs:comment "X-ray Reflectometry (XRR) measures the intensity of X-rays reflected from thin films or multilayers as a function of incident angle to determine film thickness, density, and interface roughness." ;
     rdfs:label "XRR" ;
     <http://www.w3.org/2004/02/skos/core#altLabel> "X-ray reflectivity" ,
                                                    "X-ray specular reflectivity" ;
     <http://www.w3.org/2004/02/skos/core#prefLabel> "X-ray Reflectometry" .


###  http://purl.org/pan-science/ESRFET#XRS
:XRS rdf:type owl:Class ;
     rdfs:subClassOf :experimental_technique ;
     rdfs:comment "X-ray Raman Scattering (XRS) measures inelastic scattering of hard X-rays by core electrons, enabling the study of low-Z elements’ electronic structure and bonding in bulk samples without the need for soft X-rays or vacuum conditions." ;
     rdfs:label "XRS" ;
     <http://www.w3.org/2004/02/skos/core#prefLabel> "X-ray Raman Scattering" .


###  http://purl.org/pan-science/ESRFET#XRT
:XRT rdf:type owl:Class ;
     rdfs:subClassOf :experimental_technique ;
     rdfs:comment "X-ray Diffraction Topography (XRT) records spatial variations in the intensity of X-ray diffraction from a crystal to image defects, dislocations, and strain fields with high spatial resolution, revealing crystal quality and internal microstructure." ;
     rdfs:label "XRT" ;
     <http://www.w3.org/2004/02/skos/core#altLabel> "X-ray Diffraction Topography" ,
                                                    "XDT" ;
     <http://www.w3.org/2004/02/skos/core#prefLabel> "X-ray Topography" .


###  http://purl.org/pan-science/ESRFET#XSPCI
:XSPCI rdf:type owl:Class ;
       owl:equivalentClass [ owl:intersectionOf ( :experimental_technique
                                                  [ rdf:type owl:Restriction ;
                                                    owl:onProperty :measures_as_a_function_of ;
                                                    owl:someValuesFrom <http://purl.org/pan-science/PaNET/PaNET01106>
                                                  ]
                                                  [ rdf:type owl:Restriction ;
                                                    owl:onProperty :measures_result_of_interaction ;
                                                    owl:someValuesFrom :diffusion
                                                  ]
                                                  [ rdf:type owl:Restriction ;
                                                    owl:onProperty :measures_result_of_interaction ;
                                                    owl:someValuesFrom :refraction
                                                  ]
                                                  [ rdf:type owl:Restriction ;
                                                    owl:onProperty :measures_result_of_interaction ;
                                                    owl:someValuesFrom :transmission
                                                  ]
                                                  [ rdf:type owl:Restriction ;
                                                    owl:onProperty :requires_sample_input ;
                                                    owl:someValuesFrom :x-ray
                                                  ]
                                                  [ rdf:type owl:Restriction ;
                                                    owl:onProperty :requires_sample_input_property ;
                                                    owl:someValuesFrom :speckle_pattern
                                                  ]
                                                ) ;
                             rdf:type owl:Class
                           ] ;
       rdfs:comment "X-ray Speckle Phase-Contrast Imaging (XSPCI) measures phase shifts by analyzing distortions in speckle patterns produced by a random or structured diffuser, providing 2D images with both phase and dark-field contrast. The phase contrast enhances visibility of weakly absorbing features, while the dark-field signal quantifies sample (in)homogeneity within individual detector pixels." ;
       rdfs:label "XSPCI" ;
       <http://www.w3.org/2004/02/skos/core#prefLabel> "X-ray Speckle Phase-Contrast Imaging" .


###  http://purl.org/pan-science/ESRFET#XSPCT
:XSPCT rdf:type owl:Class ;
       owl:equivalentClass [ owl:intersectionOf ( :experimental_technique
                                                  [ rdf:type owl:Restriction ;
                                                    owl:onProperty :measures_as_a_function_of ;
                                                    owl:someValuesFrom :tomography
                                                  ]
                                                  [ rdf:type owl:Restriction ;
                                                    owl:onProperty :measures_result_of_interaction ;
                                                    owl:someValuesFrom :diffusion
                                                  ]
                                                  [ rdf:type owl:Restriction ;
                                                    owl:onProperty :measures_result_of_interaction ;
                                                    owl:someValuesFrom :refraction
                                                  ]
                                                  [ rdf:type owl:Restriction ;
                                                    owl:onProperty :measures_result_of_interaction ;
                                                    owl:someValuesFrom :transmission
                                                  ]
                                                  [ rdf:type owl:Restriction ;
                                                    owl:onProperty :requires_sample_input ;
                                                    owl:someValuesFrom :x-ray
                                                  ]
                                                  [ rdf:type owl:Restriction ;
                                                    owl:onProperty :requires_sample_input_property ;
                                                    owl:someValuesFrom :speckle_pattern
                                                  ]
                                                ) ;
                             rdf:type owl:Class
                           ] ;
       rdfs:comment "X-ray Speckle Phase-Contrast Tomography (XSPCT) measures phase shifts by tracking speckle pattern distortions as the sample rotates, enabling 3D imaging of weakly absorbing materials and providing both phase and dark-field contrast, which is a measure for sample (in)homogeneity within one detector pixel." ;
       rdfs:label "XSPCT" ;
       <http://www.w3.org/2004/02/skos/core#prefLabel> "X-ray Speckle Phase-Contrast Tomography" .


###  http://purl.org/pan-science/ESRFET#absorption
:absorption rdf:type owl:Class ;
            owl:equivalentClass :atomic_core_excitation ;
            rdfs:subClassOf :cascade_of_events_being_detected .


###  http://purl.org/pan-science/ESRFET#ambient_temperature
:ambient_temperature rdf:type owl:Class ;
                     rdfs:subClassOf :sample_temperature ;
                     rdfs:comment "Reference: 20–25 °C" ,
                                  "~300 K" .


###  http://purl.org/pan-science/ESRFET#analyzer_crystal
:analyzer_crystal rdf:type owl:Class ;
                  rdfs:subClassOf :detector_type .


###  http://purl.org/pan-science/ESRFET#area_detector
:area_detector rdf:type owl:Class ;
               rdfs:subClassOf :detector_type ;
               rdfs:comment "Detector that distinguishes the position of the waves (photons or particles) in a 2D plane in space by using an array of pixels which measure the waves independently." .


###  http://purl.org/pan-science/ESRFET#atmospheric_pressure
:atmospheric_pressure rdf:type owl:Class ;
                      rdfs:subClassOf :sample_pressure ;
                      rdfs:comment "~1 × 10⁵ Pa (101 325 Pa)" .


###  http://purl.org/pan-science/ESRFET#atomic_core_excitation
:atomic_core_excitation rdf:type owl:Class ;
                        rdfs:subClassOf :cascade_of_events_being_detected ;
                        rdfs:comment "Detecting any of the results after atomic core excitation (fluorescence, photo-electrons or auger-electrons)" .


###  http://purl.org/pan-science/ESRFET#auger_electrons
:auger_electrons rdf:type owl:Class ;
                 rdfs:subClassOf :cascade_of_events_being_detected ;
                 rdfs:comment "Detecting one result after atomic core excitation (auger electrons)" .


###  http://purl.org/pan-science/ESRFET#biological_sample
:biological_sample rdf:type owl:Class ;
                   rdfs:subClassOf :sample_type ;
                   rdfs:comment "Any material taken from a living organism or made of biological molecules, such as cells, tissues, membranes, proteins, nucleic acid, DNA, or viruses" .


###  http://purl.org/pan-science/ESRFET#cascade_of_events_being_detected
:cascade_of_events_being_detected rdf:type owl:Class ;
                                  rdfs:subClassOf :technique_property ;
                                  rdfs:comment "The interaction between the sample and sample input(s) leads to a cascade of events, the result of which is being detected." .


###  http://purl.org/pan-science/ESRFET#charged_particles
:charged_particles rdf:type owl:Class ;
                   rdfs:subClassOf :sample_input ;
                   rdfs:comment "For example protons or helium ions" .


###  http://purl.org/pan-science/ESRFET#chemical_solution
:chemical_solution rdf:type owl:Class ;
                   rdfs:subClassOf :sample_type ;
                   rdfs:comment "A homogeneous mixture of solutes dissolved in a solvent." .


###  http://purl.org/pan-science/ESRFET#cryogenic_temperature
:cryogenic_temperature rdf:type owl:Class ;
                       rdfs:subClassOf :sample_temperature ;
                       rdfs:comment "1 - 77 K" ,
                                    "Liquid He (4.2 K), superconductivity, quantum devices" .


###  http://purl.org/pan-science/ESRFET#detected_cascade_of_events_property
:detected_cascade_of_events_property rdf:type owl:Class ;
                                     rdfs:subClassOf :technique_property ;
                                     rdfs:comment "The interaction between the sample and sample input(s) leads to a cascade of events, the result has properties which are being detected." .


###  http://purl.org/pan-science/ESRFET#detected_photon_property
:detected_photon_property rdf:type owl:Class ;
                          rdfs:subClassOf :detected_cascade_of_events_property ;
                          rdfs:comment "The interaction between the sample and sample input(s) leads to a cascade of events, the result being photons which properties are being measured." .


###  http://purl.org/pan-science/ESRFET#detection_as_a_function_of_incident_energy
:detection_as_a_function_of_incident_energy rdf:type owl:Class ;
                                            rdfs:subClassOf :space_time ;
                                            rdfs:comment "Detect as a function of the incident photon or particle energy" .


###  http://purl.org/pan-science/ESRFET#detection_as_a_function_of_limited_number_of_incident_energies
:detection_as_a_function_of_limited_number_of_incident_energies rdf:type owl:Class ;
                                                                rdfs:subClassOf :detection_as_a_function_of_incident_energy .


###  http://purl.org/pan-science/ESRFET#detection_as_a_function_of_limited_number_of_sample_to_detector_distance
:detection_as_a_function_of_limited_number_of_sample_to_detector_distance rdf:type owl:Class ;
                                                                          rdfs:subClassOf :detection_as_a_function_of_sample_to_detector_distance .


###  http://purl.org/pan-science/ESRFET#detection_as_a_function_of_sample_to_detector_distance
:detection_as_a_function_of_sample_to_detector_distance rdf:type owl:Class ;
                                                        rdfs:subClassOf :space_time .


###  http://purl.org/pan-science/ESRFET#detection_as_a_function_of_time
:detection_as_a_function_of_time rdf:type owl:Class ;
                                 rdfs:subClassOf :space_time ;
                                 rdfs:comment "Used to describe techniques that involve time-resolved measurements" .


###  http://purl.org/pan-science/ESRFET#detection_resolution
:detection_resolution rdf:type owl:Class ;
                      rdfs:subClassOf :detected_cascade_of_events_property ;
                      rdfs:comment "The interaction between the sample and sample input(s) leads to a cascade of events, the resolution of the certain result properties are measured." .


###  http://purl.org/pan-science/ESRFET#detector_type
:detector_type rdf:type owl:Class ;
               rdfs:subClassOf :technique_property ;
               rdfs:comment "The interaction between the sample and sample input(s) leads to a cascade of events, the result has properties which are being detected with a detector that has certain characteristics." .


###  http://purl.org/pan-science/ESRFET#diffraction
:diffraction rdf:type owl:Class ;
             rdfs:subClassOf :cascade_of_events_being_detected ;
             rdfs:comment "Detecting interference of elastically scattering photons or particles" .


###  http://purl.org/pan-science/ESRFET#diffraction_of_elastic_scattering
:diffraction_of_elastic_scattering rdf:type owl:Class ;
                                   rdfs:subClassOf :diffraction .


###  http://purl.org/pan-science/ESRFET#diffusion
:diffusion rdf:type owl:Class ;
           rdfs:subClassOf :cascade_of_events_being_detected ;
           rdfs:comment "Also referred to as \"dark-field\"." .


###  http://purl.org/pan-science/ESRFET#disperse_incident_energy_in_space
:disperse_incident_energy_in_space rdf:type owl:Class ;
                                   rdfs:subClassOf :sample_input_property ;
                                   rdfs:comment "Disperse incident wave photons in space with a polychromator (e.g. elliptically curved crystal in Bragg or Laue geometry)." .


###  http://purl.org/pan-science/ESRFET#electrons
:electrons rdf:type owl:Class ;
           rdfs:subClassOf :sample_input .


###  http://purl.org/pan-science/ESRFET#energy_dispersive_detector
:energy_dispersive_detector rdf:type owl:Class ;
                            rdfs:subClassOf :detector_type ;
                            rdfs:comment "Detector that distinguishes the energy of the waves (photons or particles) it measures with a semiconductor material which seperates energies based on the electrical current they generate in the semiconductor material." .


###  http://purl.org/pan-science/ESRFET#experimental_technique
:experimental_technique rdf:type owl:Class ;
                        rdfs:comment "A specific method or procedure used to perform experiments and gather data to investigate scientific questions." ,
                                     """Every technique has a short description that tells what we measure and what you get out of it.

In addition, experimental techniques are semantically defined by
- *what* a technique measures
- *what* inputs it requires
- *how* the measurement""" .


###  http://purl.org/pan-science/ESRFET#extended
:extended rdf:type owl:Class ;
          rdfs:subClassOf :detection_as_a_function_of_incident_energy ;
          rdfs:comment "Incident energy is scanned over a range > 200 eV" .


###  http://purl.org/pan-science/ESRFET#extreme_high_vacuum
:extreme_high_vacuum rdf:type owl:Class ;
                     rdfs:subClassOf :sample_pressure ;
                     rdfs:comment "< 1 × 10⁻¹⁰ Pa" ,
                                  "Used in fundamental physics, surface science" ;
                     <http://www.w3.org/2004/02/skos/core#altLabel> "XHV" .


###  http://purl.org/pan-science/ESRFET#extreme_pressure
:extreme_pressure rdf:type owl:Class ;
                  rdfs:subClassOf :sample_pressure ;
                  rdfs:comment "> 1 × 10¹¹ Pa" ,
                               "Planetary interiors, shock compression studies" ;
                  <http://www.w3.org/2004/02/skos/core#altLabel> "EP" .


###  http://purl.org/pan-science/ESRFET#extreme_temperature
:extreme_temperature rdf:type owl:Class ;
                     rdfs:subClassOf :sample_temperature ;
                     rdfs:comment "5,000 – 10⁷ K" ,
                                  "Fusion plasmas, stellar photospheres, inertial confinement" .


###  http://purl.org/pan-science/ESRFET#fluorescence
:fluorescence rdf:type owl:Class ;
              rdfs:subClassOf :cascade_of_events_being_detected ;
              rdfs:comment "Detecting one result after atomic core excitation (fluorescence)" .


###  http://purl.org/pan-science/ESRFET#full-field_imaging
:full-field_imaging rdf:type owl:Class ;
                    rdfs:subClassOf :imaging ;
                    rdfs:comment "Image of the sample in a single measurement (no motion of beam, sample or detector)" ,
                                 "Measure sample characteristics in a 2D plane in space by why of detection." .


###  http://purl.org/pan-science/ESRFET#grating
:grating rdf:type owl:Class ;
         rdfs:subClassOf :primary_beam_modification ;
         rdfs:comment "X-ray beam goes through an absorbing periodic structured material." .


###  http://purl.org/pan-science/ESRFET#hard_x-ray
:hard_x-ray rdf:type owl:Class ;
            rdfs:subClassOf :named_photon_energy_ranges ;
            rdfs:comment "Defined using an object property (has_photon_energy_range) to connect to another class (photon_energy_range) that has the data properties (value and unit). It creates a chain where the characteristics of other classes included in the definition define the class. Works with the reasoner!" .


###  http://purl.org/pan-science/ESRFET#high_precision_in_Q_space
:high_precision_in_Q_space rdf:type owl:Class ;
                           rdfs:subClassOf :detection_resolution ;
                           rdfs:comment """For example min(ΔQ) = 1e-4 Å-1 to 5e-4 Å-1

Angular resolution: min(Δ2θ) = 0.001° to 0.005°

Resolving power (Δ2θ/θ)""" .


###  http://purl.org/pan-science/ESRFET#high_pressure
:high_pressure rdf:type owl:Class ;
               rdfs:subClassOf :sample_pressure ;
               rdfs:comment "1 × 10⁷ – 1 × 10⁹ Pa" ,
                            "geophysics, diamond anvil cells" ;
               <http://www.w3.org/2004/02/skos/core#altLabel> "HP" .


###  http://purl.org/pan-science/ESRFET#high_temperature
:high_temperature rdf:type owl:Class ;
                  rdfs:subClassOf :sample_temperature ;
                  rdfs:comment "1,000 – 2,000 K" ,
                               "Metallurgy, refractory studies" .


###  http://purl.org/pan-science/ESRFET#high_vacuum
:high_vacuum rdf:type owl:Class ;
             rdfs:subClassOf :sample_pressure ;
             rdfs:comment "1 × 10⁻⁷ – 1 × 10⁻³ Pa" ,
                          "Thin film deposition, mass spectrometry" ;
             <http://www.w3.org/2004/02/skos/core#altLabel> "HV" .


###  http://purl.org/pan-science/ESRFET#horizontal_linear_polarization
:horizontal_linear_polarization rdf:type owl:Class ;
                                rdfs:subClassOf :polarization .


###  http://purl.org/pan-science/ESRFET#imaging
:imaging rdf:type owl:Class ;
         rdfs:subClassOf :space_time .


###  http://purl.org/pan-science/ESRFET#individual_specimen
:individual_specimen rdf:type owl:Class ;
                     rdfs:subClassOf :space_time ;
                     rdfs:comment "A method of data collection where measuring one sample providse enough data that can be analyzed. You don't necessarily need many. Although might still do it for static purposes (e.g. measuring several lungs)." .


###  http://purl.org/pan-science/ESRFET#infrared
:infrared rdf:type owl:Class ;
          rdfs:subClassOf :named_photon_energy_ranges .


###  http://purl.org/pan-science/ESRFET#laminography
:laminography rdf:type owl:Class ;
              rdfs:subClassOf :tomography ;
              rdfs:comment "Many images of the sample under different orientations from which a 3D volume can be reconstructed. The rotation axis is titled with respect to the primary beam." .


###  http://purl.org/pan-science/ESRFET#large_length_scales
:large_length_scales rdf:type owl:Class ;
                     rdfs:subClassOf :detection_resolution ;
                     rdfs:comment """Length Scale d (Å) = 10 – 1000

Q-Range (Å−1) = 0.01 – 0.1

Large structural features: supramolecular structures, particle sizes, and shapes""" .


###  http://purl.org/pan-science/ESRFET#laser
:laser rdf:type owl:Class ;
       rdfs:subClassOf :sample_input .


###  http://purl.org/pan-science/ESRFET#left_circular_polarization
:left_circular_polarization rdf:type owl:Class ;
                            rdfs:subClassOf :polarization .


###  http://purl.org/pan-science/ESRFET#low_overpressure
:low_overpressure rdf:type owl:Class ;
                  rdfs:subClassOf :sample_pressure ;
                  rdfs:comment "1 × 10⁵ – 1 × 10⁷ Pa" ,
                               "autoclaves, compressed gases" ;
                  <http://www.w3.org/2004/02/skos/core#altLabel> "LOP" .


###  http://purl.org/pan-science/ESRFET#low_temperature
:low_temperature rdf:type owl:Class ;
                 rdfs:subClassOf :sample_temperature ;
                 rdfs:comment "77 – 300 K" ,
                              "Liquid N₂ (77 K) up to room temperature (~293 K)" .


###  http://purl.org/pan-science/ESRFET#low_vacuum
:low_vacuum rdf:type owl:Class ;
            rdfs:subClassOf :sample_pressure ;
            rdfs:comment "100 – 1 × 10⁵ Pa" ,
                         "Industrial vacuum, rough pumping" ;
            <http://www.w3.org/2004/02/skos/core#altLabel> "LV" .


###  http://purl.org/pan-science/ESRFET#macro_sample_spatial_resolution
:macro_sample_spatial_resolution rdf:type owl:Class ;
                                 rdfs:subClassOf :sample_spatial_resolution ;
                                 rdfs:comment "Sample properties are measured with a resolution in space greater than 100 micron." .


###  http://purl.org/pan-science/ESRFET#magnetic_field
:magnetic_field rdf:type owl:Class ;
                rdfs:subClassOf :sample_input .


###  http://purl.org/pan-science/ESRFET#medium_vacuum
:medium_vacuum rdf:type owl:Class ;
               rdfs:subClassOf :sample_pressure ;
               rdfs:comment "1 × 10⁻³ – 100 Pa" ,
                            "Vacuum furnaces, low-pressure plasma" ;
               <http://www.w3.org/2004/02/skos/core#altLabel> "MV" .


###  http://purl.org/pan-science/ESRFET#micro_sample_spatial_resolution
:micro_sample_spatial_resolution rdf:type owl:Class ;
                                 rdfs:subClassOf :sample_spatial_resolution ;
                                 rdfs:comment "Sample properties are measured with a resolution in space between than 0.1 and 100 micron." .


###  http://purl.org/pan-science/ESRFET#moderately_high_temperature
:moderately_high_temperature rdf:type owl:Class ;
                             rdfs:subClassOf :sample_temperature ;
                             rdfs:comment "300 – 1,000 K" ,
                                          "Industrial heating, some combustion" .


###  http://purl.org/pan-science/ESRFET#monochromatic_beam
:monochromatic_beam rdf:type owl:Class ;
                    rdfs:subClassOf :photon_energy_bandwidth ;
                    rdfs:comment "Photon energy bandwidth is smaller than ???" .


###  http://purl.org/pan-science/ESRFET#multi_sample_spatial_resolution
:multi_sample_spatial_resolution rdf:type owl:Class ;
                                 rdfs:subClassOf :sample_spatial_resolution ;
                                 rdfs:comment "Detect at different resolutions." .


###  http://purl.org/pan-science/ESRFET#named_photon_energy_ranges
:named_photon_energy_ranges rdf:type owl:Class ;
                            rdfs:subClassOf :sample_input .


###  http://purl.org/pan-science/ESRFET#nano_sample_spatial_resolution
:nano_sample_spatial_resolution rdf:type owl:Class ;
                                rdfs:subClassOf :sample_spatial_resolution ;
                                rdfs:comment "Sample properties are measured with a resolution in space between than 0.1 and 100 nanometer." .


###  http://purl.org/pan-science/ESRFET#near_edge
:near_edge rdf:type owl:Class ;
           rdfs:subClassOf :detection_as_a_function_of_incident_energy ;
           rdfs:comment "Incident energy is scanned of a range <200 eV" .


###  http://purl.org/pan-science/ESRFET#photo_electrons
:photo_electrons rdf:type owl:Class ;
                 rdfs:subClassOf :cascade_of_events_being_detected ;
                 rdfs:comment "Detecting one result after atomic core excitation (photo electrons)" .


###  http://purl.org/pan-science/ESRFET#photon_count
:photon_count rdf:type owl:Class ;
              rdfs:subClassOf :detected_photon_property .


###  http://purl.org/pan-science/ESRFET#photon_direction_with_respect_to_primary_beam
:photon_direction_with_respect_to_primary_beam rdf:type owl:Class ;
                                               rdfs:subClassOf :detected_photon_property ;
                                               rdfs:comment "Not sure we need this. This was XRPD (angular dispersive) vs. ED-XRPD (energy dispersive)." .


###  http://purl.org/pan-science/ESRFET#photon_energy
:photon_energy rdf:type owl:Class ;
               rdfs:subClassOf :detected_photon_property ;
               rdfs:comment "Counting photons and their energy by semiconductors" .


###  http://purl.org/pan-science/ESRFET#photon_energy_bandwidth
:photon_energy_bandwidth rdf:type owl:Class ;
                         rdfs:subClassOf :sample_input .


###  http://purl.org/pan-science/ESRFET#pink_beam
:pink_beam rdf:type owl:Class ;
           rdfs:subClassOf :photon_energy_bandwidth ;
           rdfs:comment "Photon energy bandwidth is between ???" .


###  http://purl.org/pan-science/ESRFET#point_detector
:point_detector rdf:type owl:Class ;
                rdfs:subClassOf :detector_type ;
                rdfs:comment "Detector that cannot distinguish the position of the waves (photons or particles) in space." .


###  http://purl.org/pan-science/ESRFET#polarization
:polarization rdf:type owl:Class ;
              rdfs:subClassOf :detected_photon_property .


###  http://purl.org/pan-science/ESRFET#polycrystalline_sample
:polycrystalline_sample rdf:type owl:Class ;
                        rdfs:subClassOf :sample_type ;
                        rdfs:comment "A polycrystalline material is composed of many small single crystals (grains) with different orientations joined together." .


###  http://purl.org/pan-science/ESRFET#powder_sample
:powder_sample rdf:type owl:Class ;
               rdfs:subClassOf :sample_type ;
               rdfs:comment "A powder is a collection of tiny, separate crystalline particles with random orientations." .


###  http://purl.org/pan-science/ESRFET#primary_beam_modification
:primary_beam_modification rdf:type owl:Class ;
                           rdfs:subClassOf :sample_input_property .


###  http://purl.org/pan-science/ESRFET#ramp_compression
:ramp_compression rdf:type owl:Class ;
                  rdfs:subClassOf :sample_compression ;
                  rdfs:comment "Lower strain rates (~10^3 to 10^6 s⁻¹)" .


###  http://purl.org/pan-science/ESRFET#reflection
:reflection rdf:type owl:Class ;
            rdfs:subClassOf :cascade_of_events_being_detected ;
            rdfs:comment "Detect waves (photons or particles) which are reflected of the interface between two media." ;
            <http://www.w3.org/2004/02/skos/core#altLabel> "total reflection" .


###  http://purl.org/pan-science/ESRFET#refraction
:refraction rdf:type owl:Class ;
            rdfs:subClassOf :cascade_of_events_being_detected ;
            rdfs:comment "Detect waves (photons or particles) which are redirected as a result of passing from one medium to another." .


###  http://purl.org/pan-science/ESRFET#right_circular_polarization
:right_circular_polarization rdf:type owl:Class ;
                             rdfs:subClassOf :polarization .


###  http://purl.org/pan-science/ESRFET#sample_compression
:sample_compression rdf:type owl:Class ;
                    rdfs:subClassOf :space_time .


###  http://purl.org/pan-science/ESRFET#sample_incident_angle
:sample_incident_angle rdf:type owl:Class ;
                       rdfs:subClassOf :sample_input_property ;
                       rdfs:comment "The angle between the incident wave (photons or particles) and the sample surface." .


###  http://purl.org/pan-science/ESRFET#sample_incident_angle_smaller_than_critical_angle
:sample_incident_angle_smaller_than_critical_angle rdf:type owl:Class ;
                                                   rdfs:subClassOf :sample_incident_angle ;
                                                   rdfs:comment "The angle between the incident wave (photons or particles) and the sample surface is below the critical angle for reflection." .


###  http://purl.org/pan-science/ESRFET#sample_input
:sample_input rdf:type owl:Class ;
              rdfs:subClassOf :technique_property ;
              rdfs:comment "Everything that influences the sample during an experiment." .


###  http://purl.org/pan-science/ESRFET#sample_input_property
:sample_input_property rdf:type owl:Class ;
                       rdfs:subClassOf :technique_property ;
                       rdfs:comment "Properties of everything that influences the sample during an experiment." .


###  http://purl.org/pan-science/ESRFET#sample_pressure
:sample_pressure rdf:type owl:Class ;
                 rdfs:subClassOf :sample_input_property .


###  http://purl.org/pan-science/ESRFET#sample_spatial_resolution
:sample_spatial_resolution rdf:type owl:Class ;
                           rdfs:subClassOf :space_time .


###  http://purl.org/pan-science/ESRFET#sample_spatial_resolution_achieved_on_detection
:sample_spatial_resolution_achieved_on_detection rdf:type owl:Class ;
                                                 rdfs:subClassOf :sample_spatial_resolution ;
                                                 rdfs:comment "Sample properties are measured with a resolution in space determined by the detection mechanism (e.g. detector resolution or beam size)." ,
                                                              """achieved_on could be an object property of the  \"sample_spatial_resolution\" in this case:

\"sample_spatial_resolution\"
     achieved_on
\"detection\"

and remove this class""" .


###  http://purl.org/pan-science/ESRFET#sample_spatial_resolution_achived_on_input
:sample_spatial_resolution_achived_on_input rdf:type owl:Class ;
                                            rdfs:subClassOf :sample_spatial_resolution ;
                                            rdfs:comment "Sample properties are measured with a resolution in space determined by the sample input." .


###  http://purl.org/pan-science/ESRFET#sample_temperature
:sample_temperature rdf:type owl:Class ;
                    rdfs:subClassOf :sample_input_property .


###  http://purl.org/pan-science/ESRFET#sample_type
:sample_type rdf:type owl:Class ;
             rdfs:subClassOf :technique_property ;
             rdfs:comment "Charateristics of the sample being investigated." .


###  http://purl.org/pan-science/ESRFET#scanning_imaging
:scanning_imaging rdf:type owl:Class ;
                  rdfs:subClassOf :imaging ;
                  rdfs:comment "Image of the sample build up by many measurements (motion of beam, sample or detector)" ,
                               "Measure sample characteristics in a 2D plane in space by why of moving the sample." .


###  http://purl.org/pan-science/ESRFET#serial_screening
:serial_screening rdf:type owl:Class ;
                  rdfs:subClassOf :space_time ;
                  rdfs:comment "A method of data collection where many samples of the same kind are streaming through the sample input (e.g. X-ray beam), one at a time. Measuring only one does not provide enough data that can be analyzed, you need many." .


###  http://purl.org/pan-science/ESRFET#shock_compression
:shock_compression rdf:type owl:Class ;
                   rdfs:subClassOf :sample_compression ;
                   rdfs:comment "High strain rates (~10^6 to 10^9 s⁻¹)." .


###  http://purl.org/pan-science/ESRFET#simultanious_reference
:simultanious_reference rdf:type owl:Class ;
                        rdfs:subClassOf :space_time ;
                        rdfs:comment "Detect a reference compound or primary beam profile at the same time as measuring the actual sample." .


###  http://purl.org/pan-science/ESRFET#single_crystal_sample
:single_crystal_sample rdf:type owl:Class ;
                       rdfs:subClassOf :sample_type ;
                       rdfs:comment "A solid material in which the component atoms are arranged in a definite pattern and whose surface regularity reflects its internal symmetry." .


###  http://purl.org/pan-science/ESRFET#small_length_scales
:small_length_scales rdf:type owl:Class ;
                     rdfs:subClassOf :detection_resolution ;
                     rdfs:comment """Length Scale d (Å) = 1 – 10

Q-Range (Å−1) = 0.1 – 2.5

Small structural features: Atomic distances, crystal lattice spacings, molecular packing""" .


###  http://purl.org/pan-science/ESRFET#soft_x-ray
:soft_x-ray rdf:type owl:Class ;
            owl:equivalentClass [ owl:intersectionOf ( :named_photon_energy_ranges
                                                       [ rdf:type owl:Restriction ;
                                                         owl:onProperty :energy_range_value ;
                                                         owl:someValuesFrom [ rdf:type rdfs:Datatype ;
                                                                              owl:onDatatype xsd:float ;
                                                                              owl:withRestrictions ( [ xsd:minInclusive "5.0"^^xsd:float
                                                                                                     ]
                                                                                                   )
                                                                            ]
                                                       ]
                                                       [ rdf:type owl:Restriction ;
                                                         owl:onProperty :energy_range_unit ;
                                                         owl:hasValue "eV"
                                                       ]
                                                     ) ;
                                  rdf:type owl:Class
                                ] ;
            rdfs:subClassOf :named_photon_energy_ranges .


###  http://purl.org/pan-science/ESRFET#space_time
:space_time rdf:type owl:Class ;
            rdfs:subClassOf :technique_property ;
            rdfs:comment "Things that happen during the experiment as a function of space and time" .


###  http://purl.org/pan-science/ESRFET#speckle_pattern
:speckle_pattern rdf:type owl:Class ;
                 rdfs:subClassOf :primary_beam_modification ;
                 rdfs:comment "X-ray beam goes through a structured material (e.g. sandpaper)." .


###  http://purl.org/pan-science/ESRFET#strip_detector
:strip_detector rdf:type owl:Class ;
                rdfs:subClassOf :detector_type ;
                rdfs:comment "Detector that distinguishes the position of the waves (photons or particles) in a 1D strip (line with a certain thickness) in space by using an array of pixels which measure the waves independently." .


###  http://purl.org/pan-science/ESRFET#technique_property
:technique_property rdf:type owl:Class ;
                    rdfs:comment "A characteristic or feature that describes what an experimental technique can do, how it works, or what kind of information it provides (like resolution, sensitivity, or the type of data it collects)." ,
                                 "All the ranges of the object properties with experimental technique as domain." .


###  http://purl.org/pan-science/ESRFET#tomography
:tomography rdf:type owl:Class ;
            rdfs:subClassOf :space_time ;
            rdfs:comment "Many images of the sample under different orientations from which a 3D volume can be reconstructed" ,
                         "Measure sample characteristics is 3D by measuring characteristics in 2D or 1D projection under many orientations." .


###  http://purl.org/pan-science/ESRFET#total_electrons
:total_electrons rdf:type owl:Class ;
                 owl:equivalentClass [ rdf:type owl:Class ;
                                       owl:unionOf ( :auger_electrons
                                                     :photo_electrons
                                                   )
                                     ] ;
                 rdfs:subClassOf :cascade_of_events_being_detected ;
                 rdfs:comment "Detecting electron results after atomic core excitation (photo-electrons or auger-electrons)" .


###  http://purl.org/pan-science/ESRFET#transmission
:transmission rdf:type owl:Class ;
              rdfs:subClassOf :cascade_of_events_being_detected ;
              rdfs:comment "Detect incident photon or particles after passing through the sample without interaction" .


###  http://purl.org/pan-science/ESRFET#ultra_cryogenic_temperature
:ultra_cryogenic_temperature rdf:type owl:Class ;
                             rdfs:subClassOf :sample_temperature ;
                             rdfs:comment "< 1 K" ,
                                          "Dilution refrigerators, quantum experiments" .


###  http://purl.org/pan-science/ESRFET#ultra_extreme_temperature
:ultra_extreme_temperature rdf:type owl:Class ;
                           rdfs:subClassOf :sample_temperature ;
                           rdfs:comment "> 10⁷ K" ,
                                        "Stellar cores, thermonuclear explosions" .


###  http://purl.org/pan-science/ESRFET#ultra_high_vacuum
:ultra_high_vacuum rdf:type owl:Class ;
                   rdfs:subClassOf :sample_pressure ;
                   rdfs:comment "1 × 10⁻¹⁰ – 1 × 10⁻⁷ Pa" ,
                                "Particle accelerators, electron microscopy" ;
                   <http://www.w3.org/2004/02/skos/core#altLabel> "UHV" .


###  http://purl.org/pan-science/ESRFET#ultra_large_length_scales
:ultra_large_length_scales rdf:type owl:Class ;
                           rdfs:subClassOf :detection_resolution ;
                           rdfs:comment """Length Scale d (Å) = 1000 - 10000

Q-Range (Å−1) = 0.0001 - 0.01

Ultra Large structural features: large aggregates, clusters, and larger pores""" .


###  http://purl.org/pan-science/ESRFET#unmodified_beam
:unmodified_beam rdf:type owl:Class ;
                 rdfs:subClassOf :primary_beam_modification .


###  http://purl.org/pan-science/ESRFET#vertical_linear_polarization
:vertical_linear_polarization rdf:type owl:Class ;
                              rdfs:subClassOf :polarization .


###  http://purl.org/pan-science/ESRFET#very_high_pressure
:very_high_pressure rdf:type owl:Class ;
                    rdfs:subClassOf :sample_pressure ;
                    rdfs:comment "1 × 10⁹ – 1 × 10¹¹ Pa" ,
                                 "Deep Earth conditions, mineral physics" ;
                    <http://www.w3.org/2004/02/skos/core#altLabel> "VHP" .


###  http://purl.org/pan-science/ESRFET#very_high_temperature
:very_high_temperature rdf:type owl:Class ;
                       rdfs:subClassOf :sample_temperature ;
                       rdfs:comment "2,000 – 5,000 K" ,
                                    "Arc plasmas, re-entry heating" .


###  http://purl.org/pan-science/ESRFET#visual_spectrum
:visual_spectrum rdf:type owl:Class ;
                 rdfs:subClassOf :named_photon_energy_ranges .


###  http://purl.org/pan-science/ESRFET#wavelength_dispersive_detector
:wavelength_dispersive_detector rdf:type owl:Class ;
                                rdfs:subClassOf :detector_type ;
                                rdfs:comment "Detector that distinguishes the energy of the waves (photons or particles) it measures with a crystal monochromator which separates the energies in space." .


###  http://purl.org/pan-science/ESRFET#white_beam
:white_beam rdf:type owl:Class ;
            rdfs:subClassOf :photon_energy_bandwidth ;
            rdfs:comment "Photon energy bandwidth is greater than ???" .


###  http://purl.org/pan-science/ESRFET#x-ray
:x-ray rdf:type owl:Class ;
       rdfs:subClassOf :named_photon_energy_ranges .


###  http://purl.org/pan-science/ESRFET#3DXRD
<http://purl.org/pan-science/ESRFET#3DXRD> rdf:type owl:Class ;
                                           owl:equivalentClass [ owl:intersectionOf ( :experimental_technique
                                                                                      [ rdf:type owl:Restriction ;
                                                                                        owl:onProperty :measures_as_a_function_of ;
                                                                                        owl:someValuesFrom :tomography
                                                                                      ]
                                                                                      [ rdf:type owl:Restriction ;
                                                                                        owl:onProperty :measures_result_of_interaction ;
                                                                                        owl:someValuesFrom :diffraction_of_elastic_scattering
                                                                                      ]
                                                                                      [ rdf:type owl:Restriction ;
                                                                                        owl:onProperty :requires_sample_input ;
                                                                                        owl:someValuesFrom :x-ray
                                                                                      ]
                                                                                      [ rdf:type owl:Restriction ;
                                                                                        owl:onProperty :requires_sample_type ;
                                                                                        owl:someValuesFrom :polycrystalline_sample
                                                                                      ]
                                                                                    ) ;
                                                                 rdf:type owl:Class
                                                               ] ;
                                           rdfs:comment "3DXRD is a far field diffraction technique capable of reconstructing polycrystalline materials from the individual diffraction spots recorded in the diffraction pattern given that the crystallographic parameters of the material are known. The success of the technique is based on the ability of the individual diffraction spots to be separated. This means there is a trade off between the number of grains and the degree of strain that is measurable." ;
                                           rdfs:label "3DXRD" ;
                                           <http://www.w3.org/2004/02/skos/core#prefLabel> "3D X-ray Diffraction" .


###  http://purl.org/pan-science/ESRFET#FS‑XANES
<http://purl.org/pan-science/ESRFET#FS‑XANES> rdf:type owl:Class ;
                                              owl:equivalentClass [ owl:intersectionOf ( :experimental_technique
                                                                                         [ rdf:type owl:Restriction ;
                                                                                           owl:onProperty :measures_as_a_function_of ;
                                                                                           owl:someValuesFrom :near_edge
                                                                                         ]
                                                                                         [ rdf:type owl:Restriction ;
                                                                                           owl:onProperty :measures_as_a_function_of ;
                                                                                           owl:someValuesFrom :scanning_imaging
                                                                                         ]
                                                                                         [ rdf:type owl:Restriction ;
                                                                                           owl:onProperty :measures_interaction_result_property ;
                                                                                           owl:someValuesFrom :photon_count
                                                                                         ]
                                                                                         [ rdf:type owl:Restriction ;
                                                                                           owl:onProperty :measures_result_of_interaction ;
                                                                                           owl:someValuesFrom :atomic_core_excitation
                                                                                         ]
                                                                                         [ rdf:type owl:Restriction ;
                                                                                           owl:onProperty :requires_sample_input ;
                                                                                           owl:someValuesFrom :x-ray
                                                                                         ]
                                                                                       ) ;
                                                                    rdf:type owl:Class
                                                                  ] ;
                                              rdfs:comment "FS-XANES measures the near-edge region of the absorption spectrum across a 2D sample area using a focused X-ray beam, providing spatially resolved information on chemical state and electronic structure." ;
                                              rdfs:label "FS-XANES" ;
                                              <http://www.w3.org/2004/02/skos/core#prefLabel> "Full‑Spectral X-ray Absorption Near Edge Structure Imaging" .


###  http://purl.org/pan-science/ESRFET#TR‑SSX
<http://purl.org/pan-science/ESRFET#TR‑SSX> rdf:type owl:Class ;
                                            rdfs:subClassOf :experimental_technique ;
                                            rdfs:comment "Time-Resolved Serial Synchrotron Crystallography (TR‑SSX) measures time-dependent diffraction from a sequence of micro- or nano-crystals, each at a slightly different time-delay after reaction initiation. By combining pump–probe triggering (e.g., laser or mix-and-inject) with high-speed fixed-target delivery and fast detectors, TR‑SSX enables the reconstruction of 3D “molecular movies” that reveal structural changes in biomolecules under physiological conditions at microsecond to millisecond resolution." ;
                                            rdfs:label "TR‑SSX" ;
                                            <http://www.w3.org/2004/02/skos/core#prefLabel> "Time-Resolved Serial Synchrotron Crystallography" .


###  http://xmlns.com/foaf/0.1/Organization
<http://xmlns.com/foaf/0.1/Organization> rdf:type owl:Class .


#################################################################
#    Individuals
#################################################################

###  http://purl.org/pan-science/ESRFET#ESRF
:ESRF rdf:type owl:NamedIndividual ,
               <http://xmlns.com/foaf/0.1/Organization> ;
      rdfs:seeAlso <https://ror.org/02550n020> ;
      <http://xmlns.com/foaf/0.1/homepage> <http://www.esrf.fr> ;
      <http://xmlns.com/foaf/0.1/name> "ESRF" .


###  http://purl.org/pan-science/ESRFET#example_photon_count
:example_photon_count rdf:type owl:NamedIndividual ,
                               :photon_count .


###  http://purl.org/pan-science/ESRFET#wrong
:wrong rdf:type owl:NamedIndividual ;
       :measures_interaction_result_property :example_photon_count .


###  http://purl.org/pan-science/ESRFET#person/GKoumoutsos
<http://purl.org/pan-science/ESRFET#person/GKoumoutsos> rdf:type owl:NamedIndividual ,
                                                                 <http://xmlns.com/foaf/0.1/Person> ;
                                                        rdfs:seeAlso <http://orcid.org/0009-0000-6215-8493> ;
                                                        <http://xmlns.com/foaf/0.1/mbox> "koumoutsosgian@yahoo.gr"^^rdfs:Literal ;
                                                        <http://xmlns.com/foaf/0.1/name> "Giannis Koumoutsos" .


###  http://purl.org/pan-science/ESRFET#person/WDeNolf
<http://purl.org/pan-science/ESRFET#person/WDeNolf> rdf:type owl:NamedIndividual ,
                                                             <http://xmlns.com/foaf/0.1/Person> ;
                                                    <http://schema.org/affiliation> :ESRF ;
                                                    rdfs:seeAlso <http://orcid.org/0000-0003-2258-9402> ;
                                                    <http://xmlns.com/foaf/0.1/mbox> "dau-pydev@esrf.fr"^^rdfs:Literal ;
                                                    <http://xmlns.com/foaf/0.1/name> "Wout De Nolf" .


[ <http://xmlns.com/foaf/0.1/name> "Giannis Koumoutsos"
] .

_:genid849 <http://schema.org/affiliation> _:genid850 ;
            <http://xmlns.com/foaf/0.1/name> "Wout De Nolf" .

_:genid850 rdfs:seeAlso "https://ror.org/02550n020"^^xsd:anyURI ;
            <http://xmlns.com/foaf/0.1/homepage> "http://www.esrf.fr"^^xsd:anyURI ;
            <http://xmlns.com/foaf/0.1/name> "ESRF" .

#################################################################
#    Annotations
#################################################################

:sample_spatial_resolution rdfs:comment "Sample properties are measured with a resolution in space." .


#################################################################
#    General axioms
#################################################################

[ rdf:type owl:AllDisjointClasses ;
  owl:members ( :cascade_of_events_being_detected
                :detected_cascade_of_events_property
                :detector_type
                :sample_input
                :sample_input_property
                :sample_type
                :space_time
              )
] .


###  Generated by the OWL API (version 5.1.18) https://github.com/owlcs/owlapi/
